11/21 update

src/del/languageDEL.lean
@@ -10,6 +10,18 @@ inductive form (agents : Type) : Type
   | box  (a : agents)
          (φ : form)     : form
 
+-- form notation
+notation `⊥`:80         := form.bot
+prefix `p`:80           := form.var
+infix `&`:80            := form.and
+infix `⊃`               := form.impl
+notation `¬`:80 φ       := form.impl φ form.bot
+notation `⊤`:80         := ¬ (form.bot _)
+notation φ `∨` ψ        := form.impl (¬φ) ψ
+notation φ ↔ ψ          := form.and (form.impl φ ψ) (form.impl ψ φ)
+notation `K`:80         := form.box -- "a knows that φ"
+notation `C`:80         := λ a φ, ¬(form.box a (¬φ)) -- "φ is consistent with a's knowledge"
+
 
 inductive formPA (agents : Type) : Type
   | bot  {}                  : formPA
@@ -20,19 +32,26 @@ inductive formPA (agents : Type) : Type
             (φ : formPA)     : formPA
   | update {} (φ ψ : formPA) : formPA
 
-
--- Notation
---local notation `⊥`:80   := formPA.bot
---local prefix `p`:80     := formPA.var
+-- formPA notation
 notation `⊥`:80         := formPA.bot
 prefix `p`:80           := formPA.var
 infix `&`:80            := formPA.and
 infix `⊃`               := formPA.impl
-notation `~`:80 φ       := φ ⊃ formPA.bot
-notation `⊤`:80         := ~ (formPA.bot _)
-notation φ `∨` ψ        := ((~φ) ⊃ ψ)
-notation φ ↔ ψ          := (φ ⊃ ψ) & (ψ ⊃ φ)
+notation `¬`:80 φ       := formPA.impl φ formPA.bot
+notation `⊤`:80         := ¬ (formPA.bot _)
+notation φ `∨` ψ        := formPA.impl (¬φ) ψ
+notation φ ↔ ψ          := formPA.and (formPA.impl φ ψ) (formPA.impl ψ φ)
 notation `K`:80         := formPA.box -- "a knows that φ"
-notation `C`:80         := λ φ a, ~(K a (~φ)) -- "φ is consistent with a's knowledge"
+notation `C`:80         := λ φ a, ¬(formPA.box a (¬φ)) -- "φ is consistent with a's knowledge"
 notation `U`:80         := formPA.update
-notation `D`:80         := λ φ ψ, ~(U φ (~ψ))
+notation `D`:80         := λ φ ψ, ¬(formPA.update φ (¬ψ))
+
+
+variable {agents : Type}
+
+def to_PA : form agents → formPA agents
+  | (form.bot)      := formPA.bot
+  | (form.var n)    := formPA.var n
+  | (form.and φ ψ)  := formPA.and (to_PA φ) (to_PA ψ)
+  | (form.impl φ ψ) := formPA.impl (to_PA φ) (to_PA ψ)
+  | (form.box a φ)  := formPA.box a (to_PA φ)
