src/del/semantics/consistencyDEL.lean
@@ -3,154 +3,108 @@
 
 import del.languageDEL del.syntax.syntaxDEL 
 import del.semantics.semanticsDEL del.syntax.syntaxlemmasDEL
-import del.syntax.soundnessDEL order.zorn data.set.basic
+import del.syntax.soundnessDEL order.zorn data.set.basic data.list.basic
 local attribute [instance] classical.prop_decidable
 
-open prfPA
+open prfS5
+open S5lemma
 variables {agents : Type}
 
 
 ---------------------- Consistency ----------------------
 
-def sem_cons (AX : ctx agents) := ¬ global_sem_csq AX ⊥ 
+def sem_cons (AX : ctx agents) (F : set (frame agents)) := ¬ global_sem_csq AX F form.bot 
 attribute [class] sem_cons
 
-lemma sem_consPA : sem_cons ∅ :=
+lemma sem_consS5 : sem_cons (∅ : ctx agents) equiv_class :=
 begin
 rw sem_cons,
-rw global_sem_csq, 
-push_neg, 
-let f : frame := 
+rw global_sem_csq,
+push_neg,
+let f : frame agents := 
 { states := ℕ,
   h := ⟨0⟩,
-  rel := λ x y, x = y},
+  rel := λ a x y, x = y},
 use f, let v := λ n x, true,
-use v, let x := 42, use x,
-split, intros φ y h1, 
-exact false.elim h1, rw forces, 
-trivial 
+split,
+intro a,
+split,
+intro x,
+exact rfl,
+split,
+intros x y h1,
+exact eq.symm h1,
+intros x y z h1 h2,
+exact (rfl.congr h2).mp h1,
+use v,
+split,
+rw forces_ctx,
+intros φ x h1,
+exact false.elim h1, 
+let x := 42,
+use x,
+rw forces, 
+trivial
 end
 
--- lemma sem_consT : sem_cons T_axioms :=
--- begin
--- rw sem_cons, rw global_sem_csq,
--- push_neg,
--- let f : frame := 
--- { states := ℕ,
---   h := ⟨0⟩,
---   rel := λ x y, x = y},
--- use f, let v := λ n x, true,
--- use v, let x := 42, use x,
--- split, intros φ y h1, 
--- cases h1 with ψ h1, subst h1,
--- intro h1, apply h1 y,
--- exact rfl,
--- rw forces, trivial
--- end
-
--- lemma sem_consS4 : sem_cons S4_axioms :=
--- begin
--- rw sem_cons, rw global_sem_csq, push_neg,
--- let f : frame := 
--- { states := ℕ,
---   h := ⟨0⟩,
---   rel := λ x y, x = y},
--- use f, let v := λ n x, true,
--- use v, let x := 42, use x,
--- split, 
--- intros φ y h1,
--- rw S4_axioms at h1, cases h1,
--- cases h1 with ψ h1, subst h1,
--- intro h1, apply h1 y,
--- exact rfl,
--- cases h1 with ψ h1, subst h1,
--- intro h1, rw forces at *,
--- simp at *, rw forces, 
--- simp at *, exact h1,
--- rw forces, trivial
--- end
-
--- lemma sem_consS5 : sem_cons S5_axioms :=
--- begin
--- rw sem_cons, rw global_sem_csq, push_neg,
--- let f : frame := 
--- { states := ℕ,
---   h := ⟨0⟩,
---   rel := λ x y, x = y},
--- use f, let v := λ n x, true,
--- use v, let x := 42, use x,
--- split, 
--- intros φ y h1,
--- rw S5_axioms at h1, cases h1,
--- cases h1 with ψ h1, subst h1,
--- intro h1, apply h1 y,
--- exact rfl,
--- cases h1 with ψ h1, subst h1,
--- intro h1, rw forces at *,
--- simp at *, rw forces, 
--- exact h1,
--- rw forces, trivial
--- end
-
-
--- Any axiom system that is consistent does not prove false
-lemma nprfalse (AX : ctx agents) (hax : sem_cons AX) : ¬ prfPA AX ⊥ :=
+-- The S5 axiom system does not prove false
+lemma nprfalse (hax : sem_cons (∅ : ctx agents) equiv_class) : ¬ prfS5 (∅ : ctx agents) form.bot :=
 begin
-have h1 : ¬ global_sem_csq AX ⊥ → ¬ prfPA AX ⊥, 
-{have h2 : prfPA AX ⊥ → global_sem_csq AX ⊥, from soundnessPA AX ⊥, 
+have h1 : ¬ global_sem_csq (∅ : ctx agents) equiv_class form.bot → ¬ prfS5 ∅ form.bot,
+{have h2 := soundnessS5,
 rw ←not_imp_not at h2, exact h2},
 apply h1, exact hax
 end
 
-lemma prnot_to_notpr (φ : formPA agents) (AX : ctx agents) (hax : sem_cons AX) : 
-  prfPA AX (~φ) → ¬ prfPA AX φ :=
+lemma prnot_to_notpr (φ : form agents) (hax : sem_cons (∅ : ctx agents) equiv_class) : 
+  prfS5 ∅ (¬φ) → ¬ prfS5 ∅ φ :=
 begin
-intro h1, by_contradiction h2,
-have h3 : prfPA AX ⊥, from mp (mp pl5 contra_equiv_false) (mp (mp pl4 h2) h1),
-have h4 : ¬ prfPA AX ⊥, from nprfalse AX hax,
+intro h1, simp at *, by_contradiction h2,
+have h3 : prfS5 ∅ form.bot, from mp (mp pl5 contra_equiv_false) (mp (mp pl4 h2) h1),
+have h4 : ¬ prfS5 ∅ form.bot, from nprfalse hax,
 exact absurd h3 h4
 end 
 
-lemma pr_to_notprnot (φ : formPA agents) (AX : ctx agents) (hax : sem_cons AX) : 
-  prfPA AX φ → ¬ prfPA AX (~φ) :=
+lemma pr_to_notprnot (φ : form agents) (hax : sem_cons (∅ : ctx agents) equiv_class) : 
+  prfS5 ∅ φ → ¬ prfS5 ∅ (¬φ) :=
 begin
-have h1 : prfPA AX (~φ) → ¬ prfPA AX φ, from prnot_to_notpr φ AX hax,
+have h1 : prfS5 ∅ (¬φ) → ¬ prfS5 ∅ φ, from prnot_to_notpr φ hax,
 rw ←not_imp_not at h1, intro h2, apply h1, rw not_not, exact h2,
 end 
 
 -- finite conjunction of formulas
-def fin_conj : list (formPA agents) → formPA agents
-  | []  := ~formPA.bot
+def fin_conj : list (form agents) → form agents
+  | []  := ¬form.bot
   | (φ::φs) := φ & (fin_conj φs)
 
 -- a few helper lemmas about finite conjunctions
-lemma fin_conj_simp {Γ : ctx agents} : ∀ ψ : formPA agents, prfPA Γ (~fin_conj [ψ, ~ψ]) :=
+lemma fin_conj_simp {Γ : ctx agents} : ∀ ψ : form agents, prfS5 Γ (¬fin_conj [ψ, ¬ψ]) :=
 begin
 intro ψ, rw fin_conj, rw fin_conj, rw fin_conj,
-have h2 : (prfPA Γ (((~ψ)&(~⊥)) ↔ (~ψ)) → 
-  (prfPA Γ (~(ψ & ((~ψ)&(~⊥)))) ↔ prfPA Γ (~(ψ & (~ψ))))), 
+have h2 : (prfS5 Γ (((¬ψ)&(¬⊥)) ↔ (¬ψ)) → 
+  (prfS5 Γ (¬(ψ & ((¬ψ)&(¬⊥)))) ↔ prfS5 Γ (¬(ψ & (¬ψ))))), 
   from not_and_subst,
 simp at h2,
 specialize h2 phi_and_true, cases h2,
 exact h2_mpr not_contra
 end
 
-lemma imp_conj_imp_imp {Γ : ctx agents} {φ ψ χ : formPA agents} {L : list (formPA agents)} : 
-  prfPA Γ ((fin_conj (φ::L)) ⊃ ψ) ↔ prfPA Γ (fin_conj L ⊃ (φ ⊃ ψ)) :=
+lemma imp_conj_imp_imp {Γ : ctx agents} {φ ψ χ : form agents} {L : list (form agents)} : 
+  prfS5 Γ ((fin_conj (φ::L)) ⊃ ψ) ↔ prfS5 Γ (fin_conj L ⊃ (φ ⊃ ψ)) :=
 begin
 split, 
 intro h, dsimp [fin_conj] at h, rw and_right_imp at h, exact h,
 intro h, dsimp [fin_conj], rw and_right_imp, exact h
 end
 
-lemma fin_conj_cons_imp {Γ : ctx agents} {φ b : formPA agents} {L : list (formPA agents)} : 
- prfPA Γ (fin_conj (φ::L) ⊃ (φ ⊃ b)) → prfPA Γ (fin_conj L ⊃ (φ ⊃ b)) :=
+lemma fin_conj_cons_imp {Γ : ctx agents} {φ b : form agents} {L : list (form agents)} : 
+ prfS5 Γ (fin_conj (φ::L) ⊃ (φ ⊃ b)) → prfS5 Γ (fin_conj L ⊃ (φ ⊃ b)) :=
 begin
 intro h, rw imp_conj_imp_imp at h, rw imp_imp_iff_imp at h, exact h, exact φ,
 end
 
-lemma fin_conj_append {Γ : ctx agents} {L L' : list (formPA agents)} :
-  prfPA Γ ((fin_conj L' & fin_conj L) ↔ (fin_conj (L' ++ L))) :=
+lemma fin_conj_append {Γ : ctx agents} {L L' : list (form agents)} :
+  prfS5 Γ ((fin_conj L' & fin_conj L) ↔ (fin_conj (L' ++ L))) :=
 begin
 induction L', rw fin_conj,
 exact (mp (mp pl4 (cut (mp pl6 and_switch) (mp pl5 phi_and_true))) 
@@ -159,19 +113,21 @@ exact mp (mp pl4 (cut (mp pl5 and_commute) (imp_and_imp (mp pl5 L'_ih))))
   (cut iden (cut (imp_and_imp (mp pl6 L'_ih)) (mp pl6 and_commute)))
 end 
 
-lemma fin_conj_empty {AX : ctx agents} {L : list (formPA agents)} (hax : sem_cons AX) :
-  L = [] → ¬ prfPA AX (fin_conj L ⊃ ⊥) :=
+lemma fin_conj_empty {L : list (form agents)} 
+  (hax : sem_cons (∅ : ctx agents) equiv_class) :
+  L = [] → ¬ prfS5 ∅ (fin_conj L ⊃ ⊥) :=
 begin
 intro h1, subst h1, rw fin_conj,
-have h1 : prfPA AX (~⊥), from iden,
+have h1 : prfS5 (∅ : ctx agents) (¬(form.bot)), simp at *, exact iden,
 by_contradiction h2,
-have h3 : prfPA AX ⊥, from mp h2 h1,
-have h4 : ¬ prfPA AX ⊥, from nprfalse AX hax,
+have h3 : prfS5 ∅ form.bot, from mp h2 h1,
+have h4 : ¬ prfS5 ∅ form.bot, from nprfalse hax,
 exact absurd h3 h4
 end 
 
-lemma fin_conj_repeat_helper {AX : ctx agents} {θ : formPA agents} {L : list (formPA agents)} (hax : sem_cons AX) :
-  (∀ ψ ∈ L, ψ = θ) → prfPA AX (θ ⊃ fin_conj L) :=
+lemma fin_conj_repeat_helper {θ : form agents} {L : list (form agents)} 
+  (hax : sem_cons (∅ : ctx agents) equiv_class) :
+  (∀ ψ ∈ L, ψ = θ) → prfS5 ∅ (θ ⊃ fin_conj L) :=
 begin
 intros h1, induction L,
 exact mp pl1 iden,
@@ -181,30 +137,31 @@ specialize L_ih h2, subst h1,
 exact cut (mp double_imp pl4) (imp_and_and_imp (mp (mp pl4 iden) L_ih)),
 end
 
-lemma fin_conj_repeat {AX : ctx agents} {φ : formPA agents} {L : list (formPA agents)} (hax : sem_cons AX) :
-  (∀ ψ ∈ L, ψ = ~φ) → prfPA AX (~fin_conj L) → prfPA AX φ :=
+lemma fin_conj_repeat {φ : form agents} {L : list (form agents)}
+  (hax : sem_cons (∅ : ctx agents) equiv_class) :
+  (∀ ψ ∈ L, ψ = ¬φ) → prfS5 ∅ (¬fin_conj L) → prfS5 ∅ φ :=
 begin
 intros h1 h2, induction L,
 rw fin_conj at h2,
 have h3 := mp dne h2,
-have h4 := nprfalse AX hax,
+have h4 := nprfalse hax,
 exact absurd h3 h4,
 repeat {rw fin_conj at *}, simp at *,
 cases h1 with h1 h3, 
-have h5 : prfPA AX ((¬fin_conj L_tl) ⊃ ¬(¬φ)), from contrapos.mpr (fin_conj_repeat_helper hax h3),
+have h5 : prfS5 ∅ ((¬fin_conj L_tl) ⊃ ¬(¬φ)), from contrapos.mpr (fin_conj_repeat_helper hax h3),
 subst h1,
 exact (mp (mp pl3 (contrapos.mpr (cut h5 dne))) 
   (contrapos.mpr (cut ((demorgans.mp) (mp (mp pl6 (iff_not and_switch)) h2)) dne)))
 end
 
-lemma fin_conj_box2 {AX : ctx agents} {φ ψ : formPA agents} {a : agents} : 
-  prfPA AX (((K a φ) & K a ψ) ⊃ K a (φ & ψ)) :=
+lemma fin_conj_box2 {φ ψ : form agents} {a : agents} : 
+  prfS5 ∅ (((K a φ) & K a ψ) ⊃ K a (φ & ψ)) :=
 begin
 exact (mp double_imp (cut2 pl6 (cut pl5 (cut (mp kdist (nec pl4)) kdist))))
 end
 
-lemma fin_conj_boxn {AX : ctx agents} {L : list (formPA agents)} {a : agents} : 
-  prfPA AX ((fin_conj (list.map (K a) L)) ⊃ (K a (fin_conj L))) :=
+lemma fin_conj_boxn {L : list (form agents)} {a : agents} : 
+  prfS5 ∅ ((fin_conj (list.map (K a) L)) ⊃ (K a (fin_conj L))) :=
 begin
 induction L,
 rw fin_conj, simp at *, rw fin_conj,
@@ -216,7 +173,7 @@ exact (cut h1 fin_conj_box2)
 end
 
 
-lemma listempty {Γ : ctx agents} {L : list (formPA agents)} :
+lemma listempty {Γ : ctx agents} {L : list (form agents)} :
   (∀ φ ∈ L, φ ∈ Γ) → Γ = ∅ → L = [] := 
 begin
 intros h1 h2,
@@ -232,20 +189,20 @@ end
 
 
 -- consistency for a finite set of formulas L
-def fin_ax_consist (AX : ctx agents) (L : list (formPA agents)) := ¬ prfPA AX (fin_conj L ⊃ ⊥)
+def fin_ax_consist (L : list (form agents)) := ¬ prfS5 ∅ (fin_conj L ⊃ ⊥)
 
 
 -- consistency for an arbitrary set of formulas Γ
-def ax_consist (AX Γ : ctx agents) :=
-  ∀ L : list (formPA agents), (∀ ψ ∈ L, ψ ∈ Γ) → fin_ax_consist AX L
+def ax_consist (Γ : ctx agents) :=
+  ∀ L : list (form agents), (∀ ψ ∈ L, ψ ∈ Γ) → fin_ax_consist L
 
 
 -- Γ is maximally ax-consistent
-def max_ax_consist (AX Γ : ctx agents) := 
-  ax_consist AX Γ ∧ (∀ Γ', Γ ⊂ Γ' → ¬ ax_consist AX Γ')
+def max_ax_consist (Γ : ctx agents) := 
+  ax_consist Γ ∧ (∀ Γ', Γ ⊂ Γ' → ¬ ax_consist Γ')
 
 
-lemma max_imp_ax {AX Γ : ctx agents} : max_ax_consist AX Γ → ax_consist AX Γ :=
+lemma max_imp_ax {Γ : ctx agents} : max_ax_consist Γ → ax_consist Γ :=
 begin
 intro h1, rw max_ax_consist at h1, cases h1, exact h1_left
 end
@@ -256,19 +213,19 @@ if everything in L is in Gamma or equal to phi, and you can prove conj L ⊃ b,
 then there is a list L', such that everything in L' is in Gamma, and you can 
 prove conj L' ⊃ (phi ⊃ b)
 -/
-lemma five_helper (AX : ctx agents) : 
-  ∀ Γ : ctx agents, ∀ φ : formPA agents, ∀ L : list (formPA agents), ∀ b : formPA agents, 
-  (∀ ψ ∈ L, ψ ∈ Γ ∨ ψ = φ) → prfPA AX (fin_conj L ⊃ b) → ∃ L',
-  (∀ ψ ∈ L', ψ ∈ Γ) ∧ prfPA AX (fin_conj L' ⊃ (φ ⊃ b)) :=
+lemma five_helper : 
+  ∀ Γ : ctx agents, ∀ φ : form agents, ∀ L : list (form agents), ∀ b : form agents, 
+  (∀ ψ ∈ L, ψ ∈ Γ ∨ ψ = φ) → prfS5 ∅ (fin_conj L ⊃ b) → ∃ L',
+  (∀ ψ ∈ L', ψ ∈ Γ) ∧ prfS5 ∅ (fin_conj L' ⊃ (φ ⊃ b)) :=
 begin
 intros Γ φ L b h1 h2, 
 revert b, 
 induction L,
-{intros b h2, existsi ([] : list (formPA agents)), split, 
+{intros b h2, existsi ([] : list (form agents)), split, 
 intros ψ h3, exfalso, apply list.not_mem_nil ψ h3, 
 dsimp [fin_conj] at *, exact imp_if_imp_imp h2},
 {intros b h2,
-have h1a : ∀ (ψ : formPA agents), ψ ∈ L_tl → ψ ∈ Γ ∨ ψ = φ, 
+have h1a : ∀ (ψ : form agents), ψ ∈ L_tl → ψ ∈ Γ ∨ ψ = φ, 
   {intros ψ h2, specialize h1 ψ, 
   have h3 := list.subset_cons L_hd L_tl,
   have h4 := list.mem_cons_of_mem L_hd h2, 
@@ -277,68 +234,67 @@ specialize L_ih h1a,
 have h1b: L_hd ∈ Γ ∨ L_hd = φ, 
   {apply h1 L_hd, left, refl},
 cases h1b, 
-have h3 : prfPA AX (fin_conj L_tl ⊃ (L_hd ⊃ b)), 
+have h3 : prfS5 ∅ (fin_conj L_tl ⊃ (L_hd ⊃ b)), 
   from and_right_imp.mp h2,
 specialize L_ih (L_hd ⊃ b) h3,
-cases L_ih with L' ih, existsi (L_hd::L' : list (formPA agents)),
+cases L_ih with L' ih, existsi (L_hd::L' : list (form agents)),
 cases ih, split, intros ψ h4, cases h4, 
 subst h4, exact h1b, 
 apply ih_left ψ h4, rw imp_shift at ih_right,
 rw ←imp_conj_imp_imp at ih_right, exact ih_right,
-have h3 : prfPA AX (fin_conj (L_hd::L_tl) ⊃ b), 
+have h3 : prfS5 ∅ (fin_conj (L_hd::L_tl) ⊃ b), 
 exact h2, exact b,
 specialize L_ih (φ ⊃ b),
-have h5 : prfPA AX (fin_conj (L_hd :: L_tl) ⊃ b) → 
-  prfPA AX (fin_conj L_tl ⊃ (L_hd ⊃ b)), 
+have h5 : prfS5 ∅ (fin_conj (L_hd :: L_tl) ⊃ b) → 
+  prfS5 ∅ (fin_conj L_tl ⊃ (L_hd ⊃ b)), 
   from and_right_imp.mp,
 specialize h5 h2,
-have h6 : prfPA AX (fin_conj L_tl ⊃ (φ ⊃ b)), 
+have h6 : prfS5 ∅ (fin_conj L_tl ⊃ (φ ⊃ b)), 
   from eq.subst h1b h5,
 specialize L_ih h6, cases L_ih with L' ih, 
-cases ih, existsi (L' : list (formPA agents)), split, 
+cases ih, existsi (L' : list (form agents)), split, 
 exact ih_left, exact imp_imp_iff_imp.mp ih_right}
 end
 
 -- Lemma 5 from class notes
-lemma five (AX : ctx agents) : 
-  ∀ Γ : ctx agents, ∀ φ : formPA agents, ¬ ax_consist AX (Γ un φ) → ∃ L',
-  (∀ ψ ∈ L', ψ ∈ Γ) ∧ prfPA AX (fin_conj L' ⊃ ~φ) :=
+lemma five : 
+  ∀ Γ : ctx agents, ∀ φ : form agents, ¬ ax_consist (Γ ∪ φ) → ∃ L',
+  (∀ ψ ∈ L', ψ ∈ Γ) ∧ prfS5 ∅ (fin_conj L' ⊃ ¬φ) :=
 begin
 intro Γ, intro φ, intro h1, simp at *, rw ax_consist at h1, 
 push_neg at h1,
 cases h1 with L h1,
-have h2 : (∀ ψ ∈ L, ψ ∈ Γ ∨ ψ = φ) → prfPA AX (fin_conj L ⊃ ⊥) → ∃ L',
-  (∀ ψ ∈ L', ψ ∈ Γ) ∧ prfPA AX (fin_conj L' ⊃ (φ ⊃ ⊥)), from five_helper AX Γ φ L ⊥,
+have h2 : (∀ ψ ∈ L, ψ ∈ Γ ∨ ψ = φ) → prfS5 ∅ (fin_conj L ⊃ ⊥) → ∃ L',
+  (∀ ψ ∈ L', ψ ∈ Γ) ∧ prfS5 ∅ (fin_conj L' ⊃ (φ ⊃ ⊥)), from five_helper Γ φ L ⊥,
 cases h1,
-have h3 : (∀ (ψ : formPA agents), ψ ∈ L → ψ ∈ Γ ∨ ψ = φ), 
+have h3 : (∀ (ψ : form agents), ψ ∈ L → ψ ∈ Γ ∨ ψ = φ), 
 {intros ψ this, specialize h1_left ψ this, exact or.swap h1_left},
 specialize h2 h3, apply h2, rw fin_ax_consist at h1_right, rw not_not at h1_right,
 exact h1_right,
 end
 
 
-lemma six_helper (AX Γ : ctx agents) (h : ax_consist AX Γ) :
-max_ax_consist AX Γ → ∀ φ : formPA agents, φ ∈ Γ ∨ (~φ) ∈ Γ :=
+lemma six_helper (Γ : ctx agents) (h : ax_consist Γ) :
+max_ax_consist Γ → ∀ φ : form agents, φ ∈ Γ ∨ (¬φ) ∈ Γ :=
 begin
 intros h1 φ, rw or_iff_not_and_not, by_contradiction h2,
 cases h2 with h2l h2r, rw max_ax_consist at h1,
 cases h1 with h1l h1r, clear h, 
-have h2 := h1r (Γ un φ), have h3 := h1r (Γ un ¬φ),
-simp at h3, have h4 : ¬ax_consist AX (Γ un ¬φ), 
+have h2 := h1r (Γ ∪ φ), have h3 := h1r (Γ ∪ ¬φ),
+simp at h3, have h4 : ¬ax_consist (Γ ∪ ¬φ), 
 {apply h3, from set.ssubset_insert h2r},
-have h5 : ¬ax_consist AX (Γ un φ), 
+have h5 : ¬ax_consist (Γ ∪ φ), 
 {simp at *, apply h2, from set.ssubset_insert h2l}, 
-clear h2 h3, simp at *, have h6 := five AX Γ φ _, have h7 := five AX Γ (¬φ) _, 
-cases h6 with L' h6, cases h7 with L h7, dsimp at *, cases h6 with h6l h6r,
+clear h2 h3, simp at *, have h6 := five Γ φ _, have h7 := five Γ (¬φ) _, 
+cases h6 with L' h6, cases h7 with L h7, cases h6 with h6l h6r,
 cases h7 with h7l h7r,
-have h8 : prfPA AX ((fin_conj L' & fin_conj L) ⊃ ((¬φ) & ¬¬φ)), 
+have h8 : prfS5 ∅ ((fin_conj L' & fin_conj L) ⊃ ((¬φ) & ¬¬φ)), 
 from imp_and_and_imp (mp (mp pl4 h6r) h7r),
-simp at h8,
 rw ax_consist at h1l,
-have h12: prfPA AX ((fin_conj (L' ++ L)) ⊃ ⊥), 
+have h12: prfS5 ∅ ((fin_conj (L' ++ L)) ⊃ ⊥), 
 from cut (mp pl6 fin_conj_append) (cut h8 (mp pl5 contra_equiv_false)),
 specialize h1l (L' ++ L), rw fin_ax_consist at h1l,
-have h13: (∀ (ψ : formPA agents), ψ ∈ L' ++ L → ψ ∈ Γ), 
+have h13: (∀ (ψ : form agents), ψ ∈ L' ++ L → ψ ∈ Γ), 
 intro ψ, specialize h6l ψ, specialize h7l ψ, intro h13,
 rw list.mem_append at h13, cases h13, exact h6l h13, exact h7l h13,
 specialize h1l h13, exact absurd h12 h1l,
@@ -347,20 +303,20 @@ exact h5,
 end
 
 -- lemma 6 from class notes
-lemma six (AX Γ : ctx agents) (h : ax_consist AX Γ) :
-max_ax_consist AX Γ ↔ ∀ φ, (φ ∈ Γ ∨ (~φ) ∈ Γ) ∧ ¬(φ ∈ Γ ∧ (~φ) ∈ Γ) :=
+lemma six (Γ : ctx agents) (h : ax_consist Γ) :
+max_ax_consist Γ ↔ ∀ φ, (φ ∈ Γ ∨ (¬φ) ∈ Γ) ∧ ¬(φ ∈ Γ ∧ (¬φ) ∈ Γ) :=
 begin 
 simp, split, 
 intro h1, intro φ, 
-split, exact six_helper AX Γ h h1 φ,
+split, exact six_helper Γ h h1 φ,
 {rw ←not_and, by_contradiction h2,
 cases h2 with h2 h3,
 rw ax_consist at h,
-specialize h ([φ, ~φ]), simp at *,
-have h4 : (∀ (ψ : formPA agents), ψ = φ ∨ ψ = ~φ → ψ ∈ Γ), 
+specialize h ([φ, ¬φ]), simp at *,
+have h4 : (∀ (ψ : form agents), ψ = φ ∨ ψ = ¬φ → ψ ∈ Γ), 
 {intros ψ h4, cases h4, subst h4, exact h2, subst h4, exact h3},
 specialize h h4, rw fin_ax_consist at h, 
-have h5 : prfPA AX (~fin_conj [φ, ~φ]), from fin_conj_simp φ, 
+have h5 : prfS5 ∅ (¬fin_conj [φ, ¬φ]), from fin_conj_simp φ, 
 exact absurd h5 h},
 intro h1, rw max_ax_consist, split, exact h,
 intros Γ' h2,
@@ -371,21 +327,21 @@ apply (exists.elim h3_right), simp, intros ψ h4 h5,
 specialize h1 ψ, cases h1,
 cases h1_left,
 apply absurd h1_left h5,
-have h6 : (~ψ) ∈ Γ', from set.mem_of_subset_of_mem h3_left h1_left,
+have h6 : (¬ψ) ∈ Γ', from set.mem_of_subset_of_mem h3_left h1_left,
 rw ax_consist, 
 push_neg,
-existsi ([ψ,~ψ] : list (formPA agents)),
+existsi ([ψ,¬ψ] : list (form agents)),
 simp, split, intros φ h7, cases h7, subst h7, exact h4, 
 subst h7, exact h6, rw fin_ax_consist, rw not_not,
 exact fin_conj_simp ψ
 end
 
-lemma ex1help {AX Γ : ctx agents} {φ : formPA agents} {L L' : list (formPA agents)} :
-  (∀ ψ ∈ L, ψ ∈ Γ) → prfPA AX (fin_conj L ⊃ φ) → (∀ ψ ∈ L', ψ ∈ (insert φ Γ)) 
-  → ∃ L'' : list (formPA agents), (∀ ψ ∈ L'', ψ ∈ Γ) ∧ prfPA AX (fin_conj L'' ⊃ fin_conj L') :=
+lemma ex1help {Γ : ctx agents} {φ : form agents} {L L' : list (form agents)} :
+  (∀ ψ ∈ L, ψ ∈ Γ) → prfS5 ∅ (fin_conj L ⊃ φ) → (∀ ψ ∈ L', ψ ∈ (insert φ Γ)) 
+  → ∃ L'' : list (form agents), (∀ ψ ∈ L'', ψ ∈ Γ) ∧ prfS5 ∅ (fin_conj L'' ⊃ fin_conj L') :=
 begin
 intros h1 h2 h3, induction L',
-existsi ([] : list (formPA agents)),
+existsi ([] : list (form agents)),
 split,
 intros ψ h4, exact false.elim h4,
 exact iden,
@@ -394,7 +350,7 @@ specialize L'_ih h4,
 cases L'_ih with L'' L'_ih,
 cases L'_ih with ih1 ih2,
 cases h3, 
-existsi (L''++L : list formPA agents),
+existsi (L''++L : list (form agents)),
 split,
 simp at *, intros ψ h2,
 cases h2 with h2 h5,
@@ -402,13 +358,13 @@ exact ih1 ψ h2,
 exact h1 ψ h5,
 subst h3, 
 exact (cut (mp pl6 fin_conj_append) (cut (mp pl5 and_switch) (imp_and_and_imp (mp (mp pl4 h2) ih2)))),
-existsi (L'_hd::L'' : list formPA agents),
+existsi (L'_hd::L'' : list (form agents)),
 split, simp at *, split, exact h3, exact ih1,
 exact imp_and_imp ih2
 end
 
-lemma exercise1 {AX Γ : ctx agents} {φ : formPA agents} {L : list (formPA agents)} :
-  max_ax_consist AX Γ → (∀ ψ ∈ L, ψ ∈ Γ) → prfPA AX (fin_conj L ⊃ φ) → φ ∈ Γ :=
+lemma exercise1 {Γ : ctx agents} {φ : form agents} {L : list (form agents)} :
+  max_ax_consist Γ → (∀ ψ ∈ L, ψ ∈ Γ) → prfS5 ∅ (fin_conj L ⊃ φ) → φ ∈ Γ :=
 begin
 intros h1 h2 h3, 
 by_contradiction h4, 
@@ -431,105 +387,107 @@ specialize h1 L'' h7, apply h1,
 exact cut h8 h6
 end
 
-lemma max_dn (AX Γ : ctx agents) (h : max_ax_consist AX Γ) (φ : formPA agents) :
-  φ ∈ Γ ↔ (~~φ) ∈ Γ :=
+lemma max_dn (Γ : ctx agents) (h : max_ax_consist Γ) (φ : form agents) :
+  φ ∈ Γ ↔ (¬¬φ) ∈ Γ :=
 begin
 split, intro h1, 
-have h2 : (∀ ψ ∈ [φ], ψ ∈ Γ) → prfPA AX (fin_conj [φ] ⊃ (~~φ)) → (~~φ) ∈ Γ, from exercise1 h,
+have h2 : (∀ ψ ∈ [φ], ψ ∈ Γ) → prfS5 ∅ (fin_conj [φ] ⊃ (¬¬φ)) → (¬¬φ) ∈ Γ, from exercise1 h,
 simp at *, apply h2, exact h1,
 repeat {rw fin_conj},
 exact (cut (mp pl5 phi_and_true) dni), 
 intro h1,
-have h2 : (∀ ψ ∈ [~~φ], ψ ∈ Γ) → prfPA AX (fin_conj [~~φ] ⊃ φ) → φ ∈ Γ, from exercise1 h,
+have h2 : (∀ ψ ∈ [¬¬φ], ψ ∈ Γ) → prfS5 ∅ (fin_conj [¬¬φ] ⊃ φ) → φ ∈ Γ, from exercise1 h,
 simp at *, apply h2, exact h1,
 repeat {rw fin_conj},
 exact (cut (mp pl5 phi_and_true) dne), 
 end
 
-lemma max_boxdn (AX Γ : ctx agents) (h : max_ax_consist AX Γ) (φ : formPA agents) (a : agents) :
-  (~K a φ) ∈ Γ → (~K a (~~φ)) ∈ Γ :=
+lemma max_boxdn (Γ : ctx agents) (h : max_ax_consist Γ) (φ : form agents) (a : agents) :
+  (¬K a φ) ∈ Γ → (¬ (K a (¬¬φ))) ∈ Γ :=
 begin
 intro h1,
-have h2 : (∀ ψ ∈ [(~K a φ)], ψ ∈ Γ) → prfPA AX (fin_conj [(~ (K a) φ)] ⊃ (~K a (~~φ))) → (~K a (~~φ)) ∈ Γ, 
-  from exercise1 h,
-simp at *, apply h2, exact h1, clear h2,
+have h2 : ∀ a, (∀ ψ ∈ [¬ K a φ], ψ ∈ Γ) → prfS5 ∅ (fin_conj [¬ K a φ] ⊃ (¬ (K a (¬¬φ)))) → (¬ (K a (¬¬φ))) ∈ Γ,
+  from λ a, exercise1 h,
+simp at *, 
+specialize h2 a,
+apply h2, exact h1, clear h2,
 repeat {rw fin_conj at *},
 exact (cut (mp pl5 phi_and_true) (mp pl5 box_dn)), 
 end
 
-lemma max_notiff (AX Γ : ctx agents) (h : max_ax_consist AX Γ) (φ : formPA agents) :
-  φ ∉ Γ ↔ (~φ) ∈ Γ :=
+lemma max_notiff (Γ : ctx agents) (h : max_ax_consist Γ) (φ : form agents) :
+  φ ∉ Γ ↔ (¬φ) ∈ Γ :=
 begin
 split, intro h1,
-have h2 : ax_consist AX Γ, from max_imp_ax h, 
-have h3 : ∀ φ : formPA agents, φ ∈ Γ ∨ (~φ) ∈ Γ, from six_helper AX Γ h2 h,
+have h2 : ax_consist Γ, from max_imp_ax h, 
+have h3 : ∀ φ : form agents, φ ∈ Γ ∨ (¬φ) ∈ Γ, from six_helper Γ h2 h,
 specialize h3 φ, cases h3, exact absurd h3 h1, exact h3,
 intro h1,
-have h2 : ax_consist AX Γ, from max_imp_ax h, 
-have h3 : max_ax_consist AX Γ ↔ ∀ φ, (φ ∈ Γ ∨ (~φ) ∈ Γ) ∧ ¬(φ ∈ Γ ∧ (~φ) ∈ Γ), 
-  from six AX Γ h2,
-cases h3, specialize h3_mp h (~φ), simp at *,
+have h2 : ax_consist Γ, from max_imp_ax h, 
+have h3 : max_ax_consist Γ ↔ ∀ φ, (φ ∈ Γ ∨ (¬φ) ∈ Γ) ∧ ¬(φ ∈ Γ ∧ (¬φ) ∈ Γ), 
+  from six Γ h2,
+cases h3, specialize h3_mp h (¬φ), simp at *,
 cases h3_mp with mp1 mp2, specialize mp2 h1,
-have h4 : φ ∈ Γ ↔ (~~φ) ∈ Γ, from max_dn AX Γ h φ,
+have h4 : φ ∈ Γ ↔ (¬¬φ) ∈ Γ, from max_dn Γ h φ,
 rw ←not_iff_not at h4, cases h4, apply h4_mpr, exact mp2
 end
 
-lemma max_imp_1 {AX Γ : ctx agents} {φ ψ : formPA agents} : 
-  max_ax_consist AX Γ → (φ ∈ Γ → ψ ∈ Γ) → (φ ⊃ ψ) ∈ Γ :=
+lemma max_imp_1 {Γ : ctx agents} {φ ψ : form agents} : 
+  max_ax_consist Γ → (φ ∈ Γ → ψ ∈ Γ) → (φ ⊃ ψ) ∈ Γ :=
 begin
 intros h1 h2, rw imp_iff_not_or at h2,
 cases h2,
-have h3 : (∀ χ ∈ [~φ], χ ∈ Γ) → prfPA AX (fin_conj [~φ] ⊃ (φ ⊃ ψ)) → (φ ⊃ ψ) ∈ Γ, from exercise1 h1,
+have h3 : (∀ χ ∈ [¬φ], χ ∈ Γ) → prfS5 ∅ (fin_conj [¬φ] ⊃ (φ ⊃ ψ)) → (φ ⊃ ψ) ∈ Γ, from exercise1 h1,
 simp at *, apply h3, 
-exact (max_notiff AX Γ h1 φ).mp h2,
+exact (max_notiff Γ h1 φ).mp h2,
 repeat {rw fin_conj at *},
-have h4 : prfPA AX ((~φ) ⊃ (φ ⊃ ψ)), from and_right_imp.mp exfalso,
+have h4 : prfS5 ∅ ((¬φ) ⊃ (φ ⊃ ψ)), from and_right_imp.mp exfalso,
 exact cut (mp pl5 phi_and_true) h4,
-have h3 : (∀ χ ∈ [ψ], χ ∈ Γ) → prfPA AX (fin_conj [ψ] ⊃ (φ ⊃ ψ)) → (φ ⊃ ψ) ∈ Γ, from exercise1 h1,
+have h3 : (∀ χ ∈ [ψ], χ ∈ Γ) → prfS5 ∅ (fin_conj [ψ] ⊃ (φ ⊃ ψ)) → (φ ⊃ ψ) ∈ Γ, from exercise1 h1,
 simp at *, 
 apply h3, exact h2, exact (cut (mp pl5 phi_and_true) pl1),
 end
 
-lemma max_imp_2 {AX Γ : ctx agents} {φ ψ : formPA agents} : 
-  max_ax_consist AX Γ → (φ ⊃ ψ) ∈ Γ → φ ∈ Γ → ψ ∈ Γ :=
+lemma max_imp_2 {Γ : ctx agents} {φ ψ : form agents} : 
+  max_ax_consist Γ → (φ ⊃ ψ) ∈ Γ → φ ∈ Γ → ψ ∈ Γ :=
 begin
 intros h1 h2 h3,
-have h4 : (∀ χ ∈ [φ, (φ ⊃ ψ)], χ ∈ Γ) → prfPA AX (fin_conj [φ, (φ ⊃ ψ)] ⊃ ψ) → ψ ∈ Γ, from exercise1 h1,
+have h4 : (∀ χ ∈ [φ, (φ ⊃ ψ)], χ ∈ Γ) → prfS5 ∅ (fin_conj [φ, (φ ⊃ ψ)] ⊃ ψ) → ψ ∈ Γ, from exercise1 h1,
 simp at *, apply h4, intros χ h5, cases h5, subst h5, exact h3, subst h5, exact h2,
 repeat {rw fin_conj},
 exact and_right_imp.mpr (mp pl5 phi_and_true)
 end
 
-lemma max_conj_1 {AX Γ : ctx agents} {φ ψ : formPA agents} : 
-  max_ax_consist AX Γ → (φ ∈ Γ ∧ ψ ∈ Γ) → (φ & ψ) ∈ Γ :=
+lemma max_conj_1 {Γ : ctx agents} {φ ψ : form agents} : 
+  max_ax_consist Γ → (φ ∈ Γ ∧ ψ ∈ Γ) → (φ & ψ) ∈ Γ :=
 begin
 intros h1 h2, cases h2,
-have h3 : (∀ χ ∈ [φ], χ ∈ Γ) → prfPA AX (fin_conj [φ] ⊃ (ψ ⊃ (φ & ψ))) → (ψ ⊃ (φ & ψ)) ∈ Γ, 
+have h3 : (∀ χ ∈ [φ], χ ∈ Γ) → prfS5 ∅ (fin_conj [φ] ⊃ (ψ ⊃ (φ & ψ))) → (ψ ⊃ (φ & ψ)) ∈ Γ, 
   from exercise1 h1,
 simp at *, specialize h3 h2_left,
 repeat {rw fin_conj at *},
-have h5 : prfPA AX ((φ&~⊥)⊃(ψ⊃φ&ψ)),
+have h5 : prfS5 ∅ ((φ&¬⊥)⊃(ψ⊃φ&ψ)),
 exact (cut (mp pl5 phi_and_true) pl4), 
 specialize h3 h5,
 have h6 : (ψ ⊃ (φ & ψ)) ∈ Γ → ψ ∈ Γ → (φ & ψ) ∈ Γ, from max_imp_2 h1,
 apply h6, exact h3, exact h2_right
 end
 
-lemma max_conj_2 {AX Γ : ctx agents} {φ ψ : formPA agents} : 
-  max_ax_consist AX Γ → (φ & ψ) ∈ Γ → φ ∈ Γ :=
+lemma max_conj_2 {Γ : ctx agents} {φ ψ : form agents} : 
+  max_ax_consist Γ → (φ & ψ) ∈ Γ → φ ∈ Γ :=
 begin
 intros h1 h2,
-have h3 : (∀ χ ∈ [(φ & ψ)], χ ∈ Γ) → prfPA AX (fin_conj [(φ & ψ)] ⊃ φ) → φ ∈ Γ, 
+have h3 : (∀ χ ∈ [(φ & ψ)], χ ∈ Γ) → prfS5 ∅ (fin_conj [(φ & ψ)] ⊃ φ) → φ ∈ Γ, 
   from exercise1 h1,
 simp at *, apply h3, exact h2, repeat {rw fin_conj},
 exact (cut (mp pl5 phi_and_true) pl5)
 end
 
-lemma max_conj_3 {AX Γ : ctx agents} {φ ψ : formPA agents} : 
-  max_ax_consist AX Γ → (φ & ψ) ∈ Γ → ψ ∈ Γ :=
+lemma max_conj_3 {Γ : ctx agents} {φ ψ : form agents} : 
+  max_ax_consist Γ → (φ & ψ) ∈ Γ → ψ ∈ Γ :=
 begin
 intros h1 h2,
-have h3 : (∀ χ ∈ [(φ & ψ)], χ ∈ Γ) → prfPA AX (fin_conj [(φ & ψ)] ⊃ ψ) → ψ ∈ Γ, 
+have h3 : (∀ χ ∈ [(φ & ψ)], χ ∈ Γ) → prfS5 ∅ (fin_conj [(φ & ψ)] ⊃ ψ) → ψ ∈ Γ, 
   from exercise1 h1,
 simp at *, apply h3, exact h2, repeat {rw fin_conj},
 exact (cut (mp pl5 phi_and_true) pl6)
@@ -537,8 +495,8 @@ end
 
 -- Γ is maximally AX-consistent iff it is AX-consistent and for 
 -- every AX-consistent set Γ', if Γ ⊆ Γ', then Γ = Γ'
-lemma max_equiv (AX Γ : ctx agents) : max_ax_consist AX Γ ↔ ax_consist AX Γ ∧ 
-  ∀ Γ', ax_consist AX Γ' → Γ ⊆ Γ' → Γ = Γ' :=
+lemma max_equiv (Γ : ctx agents) : max_ax_consist Γ ↔ ax_consist Γ ∧ 
+  ∀ Γ', ax_consist Γ' → Γ ⊆ Γ' → Γ = Γ' :=
 begin
 split, 
 {intro h1, split, rw max_ax_consist at h1, exact h1.left, 
@@ -558,17 +516,9 @@ open zorn
 -- Lemma: if c is a chain of sets, L is a list of elements such that 
 -- every element in L is in Union(c), then there is an element m in c such that every 
 -- element of L is in m.
--- by induction on L.
--- S := collection of max cons sets
--- m := Γ'
-lemma lindenhelper (c : set (ctx agents)) (h : c.nonempty) (h1 : chain (⊆) c) (L : list (formPA agents)) :
+lemma lindenhelper (c : set (ctx agents)) (h : c.nonempty) (h1 : chain (⊆) c) (L : list (form agents)) :
 (∀ φ ∈ L, φ ∈ ⋃₀(c)) → ∃ m ∈ c, (∀ ψ ∈ L, ψ ∈ m) :=
 begin
--- have H : c = ∅ ∨ c ≠ ∅, from dec_em (c = ∅),
--- cases H, subst H,
--- have h := listempty,
--- intro h2,
--- specialize h h2, simp at *, subst h, simp at *, 
 intro h2,
 induction L, simp,
 rw ←set.nonempty_def, exact h,
@@ -582,52 +532,65 @@ simp at h2,
 cases h2 with m' h2,
 cases h2 with h2 h4,
 existsi (m' ∪ m : ctx agents), 
-have H : m' ∪ m ∈ c, 
-sorry,
-existsi (H : m' ∪ m ∈ c),
-intros ψ h5, cases h5,
-subst h5, exact set.mem_union_left m h4,
-specialize ih ψ h5, exact set.mem_union_right m' ih
+have h5 : m' ∪ m ∈ c, 
+{have h6 := chain.total_of_refl h1 h3 h2,
+cases h6,
+have h7 := set.union_eq_self_of_subset_right h6,
+exact (eq.substr h7 h2), 
+have h7 := set.union_eq_self_of_subset_left h6,
+exact (eq.substr h7 h3)},
+existsi (h5 : m' ∪ m ∈ c),
+intros ψ h6, cases h6,
+subst h6, exact set.mem_union_left m h4,
+specialize ih ψ h6, exact set.mem_union_right m' ih
 end
 
 
-lemma lindenbaum (AX Γ : ctx agents) (hax : ax_consist AX Γ) : 
-  ∃ Γ', max_ax_consist AX Γ' ∧ Γ ⊆ Γ' :=
+lemma lindenbaum (Γ : ctx agents) (hax : ax_consist Γ) : 
+  ∃ Γ', max_ax_consist Γ' ∧ Γ ⊆ Γ' :=
 begin
-let P := { Γ'' | Γ'' ⊇ Γ ∧ ax_consist AX Γ''},
-have h : ∀ c ⊆ P, chain (⊆) c → ∃ub ∈ P, ∀ s ∈ c, s ⊆ ub, 
-{intros c h1 h2, use ⋃₀(c), 
-split,
-have h3 := lindenhelper c sorry h2,
+let P := { Γ'' | Γ'' ⊇ Γ ∧ ax_consist Γ''},
+have h : ∀ c ⊆ P, chain (⊆) c → c.nonempty → ∃ub ∈ P, ∀ s ∈ c, s ⊆ ub, 
+{intros c h2 h3 h4, use ⋃₀(c), 
+have h5 := lindenhelper c h4 h3,
 split, 
-rw superset, 
-sorry,
-rw ax_consist,
-intros L h4,
-specialize h3 L h4,
-cases h3 with m h3,
-cases h3 with h5 h3,
-have h6 : m ∈ P, from set.mem_of_mem_of_subset h5 h1,
-simp at *,
+split,
+rw superset,
+rw set.nonempty_def at h4,
+cases h4 with Γ'' h4,
+have h6 := set.mem_of_mem_of_subset h4 h2,
 cases h6 with h6 h7,
-rw ax_consist at h7, apply h7, exact h3,
-intros s h3, exact set.subset_sUnion_of_mem h3
-},
-cases zorn_subset P h with Γ' h1, cases h1 with h1 h2,
-use Γ', split, rw max_equiv, split, apply h1.2, 
-intros m h3 h4, symmetry, apply h2 m, split, apply set.subset.trans h1.1 h4,
-exact h3, exact h4, apply h1.1
+rw superset at h6,
+apply set.subset_sUnion_of_subset c Γ'' h6 h4,
+rw ax_consist,
+intros L h6,
+specialize h5 L h6,
+cases h5 with m h5,
+cases h5 with h7 h5,
+have h8 := set.mem_of_mem_of_subset h7 h2,
+cases h8 with h8 h9,
+rw ax_consist at h9, apply h9, exact h5,
+intros s h7, exact set.subset_sUnion_of_mem h7},
+have h1 : Γ ∈ P,
+split,
+exact set.subset.rfl,
+exact hax,
+cases zorn_subset₀ P h Γ h1 with Γ' h2,
+cases h2 with h2 h3,
+cases h3 with h3 h4,
+use Γ', split, rw max_equiv, split, apply h2.2, 
+intros m h5 h6, symmetry, apply h4 m, split, apply set.subset.trans h2.1 h6,
+exact h5, exact h6, apply h2.1
 end
-
 
 -- Corollary 8
-lemma max_ax_exists (AX : ctx agents) (hax : sem_cons AX) : ∃ Γ : ctx agents, max_ax_consist AX Γ :=
+lemma max_ax_exists (hax : sem_cons (∅ : ctx agents) equiv_class) : ∃ Γ : ctx agents, max_ax_consist Γ :=
 begin
-have h1 : ax_consist AX ∅,
+have h1 : ax_consist ∅,
 {rw ax_consist, intro L, intro h2, rw fin_ax_consist, 
 have h3 := listempty h2, have this : ∅ = ∅, refl, 
 specialize h3 this, subst h3, by_contradiction h4, 
-have h5 := mp dne, apply nprfalse AX hax, exact h5 h4},
-have h2 : ∃ Γ, max_ax_consist AX Γ ∧ ∅ ⊆ Γ, from lindenbaum AX ∅ h1, 
+have h5 := mp dne, apply nprfalse hax, exact h5 h4},
+have h2 : ∃ Γ, max_ax_consist Γ ∧ ∅ ⊆ Γ, from lindenbaum ∅ h1, 
 cases h2 with Γ h2, cases h2 with h2 h3, existsi (Γ : ctx agents), apply h2
 end
