src/del/semantics/semanticsDEL.lean
@@ -2,18 +2,22 @@
 -- Hans van Ditmarsch, Wiebe van der Hoek, and Barteld Kooi
 
 import del.languageDEL del.syntax.syntaxDEL data.set.basic
-variable {agents : Type}
+import del.semantics.translationfunction
+
 open formPA 
+open form
+open set
 local attribute [instance] classical.prop_decidable
 
 
 ---------------------- Semantics ----------------------
 
+variable {agents : Type}
+
 structure frame (agents : Type) :=
 (states : Type)
 (h : nonempty states)
 (rel : agents → states → states → Prop)
-
 
 def frame.restrict (f : frame agents) (P : f.states → Prop) (s : f.states) (Ps : P s) : frame agents :=
 {
@@ -22,71 +26,231 @@ def frame.restrict (f : frame agents) (P : f.states → Prop) (s : f.states) (Ps
   rel := λ a : agents, λ u v, f.rel a u.val v.val
 }
 
--- definition of forces
-def forces : ∀ f : frame agents, 
-  (nat → f.states → Prop) → f.states → formPA agents → Prop
-  | f v x bot          := false
-  | f v x (var n)      := v n x
-  | f v x (and φ ψ)    := (forces f v x φ) ∧ (forces f v x ψ)
-  | f v x (impl φ ψ)   := (forces f v x φ) → (forces f v x ψ)
-  | f v x (box a φ)    := ∀ y, f.rel a x y → forces f v y φ
-  | f v x (update φ ψ) := ∀ h : forces f v x φ, 
-      forces (f.restrict (λ y, forces f v y φ) x h) (λ n u, v n u.val) ⟨x, h⟩ ψ
-
--- φ is valid in a model M = (f,v)
-def m_valid (φ : formPA agents) (f : frame agents) 
-  (v : nat → f.states → Prop) := 
-  ∀ x, forces f v x φ
-
--- valid in a frame f
-def f_valid (φ : formPA agents) (f : frame agents) := 
-  ∀ v x, forces f v x φ
-
--- φ is valid in a class of frames F = set f
-def F_valid (φ : formPA agents) (F : set (frame agents)) := 
-  ∀ f ∈ F, ∀ v x, forces f v x φ
-
--- -- φ is universally valid (valid in all frames)
--- def u_valid (φ : formPA agents) := 
---   ∀ f v x, forces f v x φ
-
--- A context is true at a world in a model if each 
--- formula of the context is true at that world in that model
-def forces_ctx (f : frame agents) (v : nat → f.states → Prop) 
-  (Γ : ctx agents) := ∀ φ, ∀ x, φ ∈ Γ → forces f v x φ
-
--- Local semantic consequence
-def local_sem_csq (Γ : ctx agents) (φ : formPA agents) :=
-  ∀ f v x, forces_ctx f v Γ → forces f v x φ
-
--- Global semantic consequence
-def global_sem_csq (Γ : ctx agents) (φ : formPA agents) :=
-  ∀ f v x, forces_ctx f v Γ → forces f v x φ
-
-
-open set
-variables (f : frame agents) {α : Type} (a : agents) (r : α → α → Prop)
+variables {α : Type} 
+variables (r : α → α → Prop)
 
 def euclidean := ∀ ⦃x y z⦄, r x y → r x z → r y z 
-
---def ref_class : set (frame agents) := { f : frame agents | ∀ a : agents, reflexive (f.rel a) }
---def symm_class : set (frame agents) := { f : frame agents | ∀ a : agents, symmetric (f.rel a) }
---def trans_class : set (frame agents ) := { f : frame agents | ∀ a : agents, transitive (f.rel a) }
 def euclid_class : set (frame agents ) := { f : frame agents | ∀ a : agents, euclidean (f.rel a) }
---def ref_trans_class : set (frame agents) := ref_class ∩ trans_class
+def ref_class : set (frame agents) := { f : frame agents | ∀ a : agents, reflexive (f.rel a) }
 def equiv_class : set (frame agents) := { f : frame agents | ∀ a : agents, equivalence (f.rel a) }
 
 
-lemma not_forces_imp (f : frame agents) : ∀ v x φ, 
-  (¬(forces f v x φ)) ↔ (forces f v x (~φ)) :=
+-- definition of forces for public announcement logic
+def forcesPA : ∀ f : frame agents, 
+  (nat → f.states → Prop) → f.states → formPA agents → Prop
+  | f v x bot          := false
+  | f v x (var n)      := v n x
+  | f v x (and φ ψ)    := (forcesPA f v x φ) ∧ (forcesPA f v x ψ)
+  | f v x (impl φ ψ)   := (forcesPA f v x φ) → (forcesPA f v x ψ)
+  | f v x (box a φ)    := ∀ y, f.rel a x y → forcesPA f v y φ
+  | f v x (update φ ψ) := ∀ h : forcesPA f v x φ, 
+      forcesPA (f.restrict (λ y, forcesPA f v y φ) x h) (λ n u, v n u.val) ⟨x, h⟩ ψ
+
+-- φ is valid in a model M = (f,v)
+def m_validPA (φ : formPA agents) (f : frame agents) 
+  (v : nat → f.states → Prop) := 
+  ∀ x, forcesPA f v x φ
+
+-- valid in a frame f
+def f_validPA (φ : formPA agents) (f : frame agents) := 
+  ∀ v x, forcesPA f v x φ
+
+-- φ is valid in a class of frames F
+def F_validPA (φ : formPA agents) (F : set (frame agents)) := 
+  ∀ f ∈ F, ∀ v x, forcesPA f v x φ
+
+-- A context is true at a world in a model if each 
+-- formula of the context is true at that world in that model
+def forces_ctxPA (f : frame agents) (v : nat → f.states → Prop) 
+  (Γ : ctxPA agents) := ∀ φ, ∀ x, φ ∈ Γ → forcesPA f v x φ
+
+-- Global semantic consequence
+def global_sem_csqPA (Γ : ctxPA agents) (F : set (frame agents)) (φ : formPA agents) :=
+  ∀ f ∈ F, ∀ v, forces_ctxPA f v Γ → ∀ x, forcesPA f v x φ
+
+
+lemma not_forces_impPA (f : frame agents) : ∀ v x φ, 
+  (¬(forcesPA f v x φ)) ↔ (forcesPA f v x (¬φ)) :=
 begin
 intros v x φ, split, 
 {intros h1 h2, exact h1 h2},
 {intros h1 h2, specialize h1 h2, exact h1}
 end
 
-lemma forces_exists {a : agents} {f : frame agents} {v : nat → f.states → Prop} {x : f.states} {φ : formPA agents} :
-  forces f v x (~K a ~φ) ↔ ∃ y : f.states, (f.rel a x y ∧ forces f v y φ) :=
+lemma forces_existsPA {a : agents} {f : frame agents} {v : nat → f.states → Prop} {x : f.states} {φ : formPA agents} :
+  forcesPA f v x (¬K a ¬φ) ↔ ∃ y : f.states, (f.rel a x y ∧ forcesPA f v y φ) :=
+begin
+split,
+intro h1,
+rw forcesPA at h1, rw forcesPA at h1,
+have h2 := not_or_of_imp h1,
+clear h1, cases h2, push_neg at h2,
+cases h2 with y h2, cases h2 with h2 h3,
+existsi (y : f.states), split, exact h2,
+have h4 := (not_forces_impPA f v y (¬φ)).mp h3,
+repeat {rw forcesPA at h4}, repeat {rw imp_false at h4},
+rw not_not at h4, exact h4,
+rw forcesPA at h2, exact false.elim h2,
+intro h1, cases h1 with y h1,
+cases h1 with h1 h2,
+rw forcesPA,
+intro h3,
+rw forcesPA at h3, specialize h3 y h1,
+rw ←not_forces_impPA at h3, 
+exact absurd h2 h3
+end
+
+lemma forces_update_dual (φ ψ : formPA agents) (f : frame agents) (v : nat → f.states → Prop) (x : f.states) : 
+forcesPA f v x ¬(U φ (¬ψ)) ↔ ∃ h : forcesPA f v x φ, 
+      forcesPA (f.restrict (λ y, forcesPA f v y φ) x h) (λ n u, v n u.val) ⟨x, h⟩ ψ :=
+begin
+split,
+{intro h1, rw forcesPA at h1, rw forcesPA at h1,
+rw forcesPA at h1, rw imp_false at h1,
+push_neg at h1,
+cases h1 with Ph1 h1, 
+existsi (Ph1 : forcesPA f v x φ), rw not_forces_impPA at h1, 
+rw forcesPA at h1, rw forcesPA at h1,
+rw forcesPA at h1, rw imp_false at h1, 
+push_neg at h1,
+cases h1 with Ph2 h2, exact Ph2},
+{intro h1, cases h1 with Ph1 h1, 
+intro h2, apply h2, exact h1}
+end
+
+lemma forcesPA_translate (f : frame agents) (v : nat → f.states → Prop) 
+  (x : f.states) (φ : formPA agents) : forcesPA f v x φ ↔ forcesPA f v x (to_PA (translate φ)) :=
+begin
+induction φ generalizing x,
+repeat {split},
+repeat {intro h1, exact h1},
+repeat {rename φ_φ φ},
+repeat {rename φ_ψ ψ},
+repeat {rename φ_ih_φ ih_φ},
+repeat {rename φ_ih_ψ ih_ψ},
+repeat {rename φ_a a},
+intro h1, rw translate,
+cases h1 with h1 h2,
+split,
+exact (ih_φ x).mp h1, exact (ih_ψ x).mp h2,
+intro h1, rw translate at h1,
+cases h1 with h1 h2,
+split,
+exact (ih_φ x).mpr h1, exact (ih_ψ x).mpr h2,
+intro h1, rw translate, intro h2,
+exact (ih_ψ x).mp (h1 ((ih_φ x).mpr h2)),
+intro h1, rw translate at h1,
+intro h2,
+exact (ih_ψ x).mpr (h1 ((ih_φ x).mp h2)),
+intro h1, rw translate, rw to_PA,
+intros y h2,
+rw forcesPA at h1,
+specialize h1 y h2,
+specialize φ_ih y, exact φ_ih.mp h1,
+intro h1, rw translate at h1, rw to_PA at h1,
+intros y h2,
+rw forcesPA at h1,
+specialize h1 y h2,
+specialize φ_ih y, exact φ_ih.mpr h1,
+induction ψ, 
+repeat {rename ψ_φ ψ},
+repeat {rename ψ_ψ χ},
+repeat {rename ψ_ih_φ ih_ψ},
+repeat {rename ψ_ih_ψ ih_χ},
+repeat {intro h1, repeat {rw translate},
+repeat {rw to_PA}, 
+intro h2,
+have h3 := (ih_φ x).mpr h2,
+specialize h1 h3,
+exact h1},
+repeat {sorry},
+end
+
+-- definition of forces for basic modal language indexed over agents...
+-- used for typeclass inference between systems
+def forces : ∀ f : frame agents, 
+  (nat → f.states → Prop) → f.states → form agents → Prop
+  | f v x form.bot          := false
+  | f v x (form.var n)      := v n x
+  | f v x (form.and φ ψ)    := (forces f v x φ) ∧ (forces f v x ψ)
+  | f v x (form.impl φ ψ)   := (forces f v x φ) → (forces f v x ψ)
+  | f v x (form.box a φ)    := ∀ y, f.rel a x y → forces f v y φ
+
+lemma forcesPA_iff_forces (φ : form agents) (f : frame agents) : 
+  ∀ v x, forcesPA f v x (to_PA φ) ↔ forces f v x φ :=
+begin
+intros v x, induction φ generalizing x,
+split,
+repeat {intro h1,
+apply h1},
+split,
+repeat {intro h1,
+apply h1},
+rename φ_ih_φ ih_φ,
+rename φ_ih_ψ ih_ψ,
+specialize ih_φ x,
+specialize ih_ψ x,
+cases ih_φ, cases ih_ψ,
+split,
+intro h1,
+cases h1 with h1 h2,
+split,
+exact ih_φ_mp h1,
+exact ih_ψ_mp h2,
+intro h1,
+cases h1 with h1 h2,
+split,
+exact ih_φ_mpr h1,
+exact ih_ψ_mpr h2,
+rename φ_ih_φ ih_φ,
+rename φ_ih_ψ ih_ψ,
+specialize ih_φ x,
+specialize ih_ψ x,
+cases ih_φ, cases ih_ψ,
+split,
+intros h1 h2,
+specialize ih_φ_mpr h2,
+specialize h1 ih_φ_mpr,
+exact ih_ψ_mp h1,
+intros h1 h2,
+specialize ih_φ_mp h2,
+specialize h1 ih_φ_mp,
+exact ih_ψ_mpr h1,
+split,
+intros h1 y h3,
+specialize h1 y h3,
+specialize φ_ih y,
+cases φ_ih,
+exact φ_ih_mp h1,
+intros h1 y h3,
+specialize h1 y h3,
+specialize φ_ih y,
+cases φ_ih,
+exact φ_ih_mpr h1
+end
+
+def F_valid (φ : form agents) (F : set (frame agents)) := 
+  ∀ f ∈ F, ∀ v x, forces f v x φ
+
+-- A context is true at a world in a model if each 
+-- formula of the context is true at that world in that model
+def forces_ctx (f : frame agents) (v : nat → f.states → Prop) 
+  (Γ : ctx agents) := ∀ φ : form agents, ∀ x, φ ∈ Γ → forces f v x φ
+
+-- global semantic consequence
+def global_sem_csq (Γ : ctx agents) (F : set (frame agents)) (φ : form agents) :=
+  ∀ f ∈ F, ∀ v, forces_ctx f v Γ → ∀ x, forces f v x φ
+
+lemma not_forces_imp (f : frame agents) : ∀ v x φ, 
+  (¬(forces f v x φ)) ↔ (forces f v x (¬φ)) :=
+begin
+intros v x φ, split, 
+{intros h1 h2, exact h1 h2},
+{intros h1 h2, specialize h1 h2, exact h1}
+end
+
+lemma forces_exists {a : agents} {f : frame agents} {v : nat → f.states → Prop} {x : f.states} {φ : form agents} :
+  forces f v x (¬K a ¬φ) ↔ ∃ y : f.states, (f.rel a x y ∧ forces f v y φ) :=
 begin
 split,
 intro h1,
@@ -95,33 +259,42 @@ have h2 := not_or_of_imp h1,
 clear h1, cases h2, push_neg at h2,
 cases h2 with y h2, cases h2 with h2 h3,
 existsi (y : f.states), split, exact h2,
-have h4 := (not_forces_imp f v y (~φ)).mp h3,
+have h4 := (not_forces_imp f v y (¬φ)).mp h3,
 repeat {rw forces at h4}, repeat {rw imp_false at h4},
 rw not_not at h4, exact h4,
-rw forces at h2, exact false.elim h2,
+exact false.elim h2,
 intro h1, cases h1 with y h1,
 cases h1 with h1 h2,
-rw forces,
 intro h3,
-rw forces at h3, specialize h3 y h1,
+specialize h3 y h1,
 rw ←not_forces_imp at h3, 
 exact absurd h2 h3
 end
 
-lemma forces_update_dual (φ ψ : formPA agents) (f : frame agents) (v : nat → f.states → Prop) (x : f.states) : 
-forces f v x ~(U φ (~ψ)) ↔ ∃ h : forces f v x φ, 
-      forces (f.restrict (λ y, forces f v y φ) x h) (λ n u, v n u.val) ⟨x, h⟩ ψ :=
+lemma equiv_ref_euclid (f : frame agents) : 
+  f ∈ (equiv_class : set (frame agents)) ↔ f ∈ ((ref_class : set (frame agents)) ∩ (euclid_class : set (frame agents))) :=
 begin
+rw equiv_class, rw ref_class, rw euclid_class,
+rw set.mem_set_of_eq, simp, split,
+intro h1,
 split,
-{intro h1, rw forces at h1, rw forces at h1,
-rw forces at h1, rw imp_false at h1,
-push_neg at h1,
-cases h1 with Ph1 h1, 
-existsi (Ph1 : forces f v x φ), rw not_forces_imp at h1, 
-rw forces at h1, rw forces at h1,
-rw forces at h1, rw imp_false at h1, 
-push_neg at h1,
-cases h1 with Ph2 h2, exact Ph2},
-{intro h1, cases h1 with Ph1 h1, 
-intro h2, apply h2, exact h1}
+intro a,
+specialize h1 a,
+cases h1 with h1 h2, cases h2 with h2 h3,
+exact h1,
+intro a, rw euclidean, intros x y z h4 h5,
+specialize h1 a, rw equivalence at h1,
+cases h1 with h1 h2, cases h2 with h2 h3,
+rw symmetric at h2, specialize h2 h4, 
+rw transitive at h3, exact h3 h2 h5,
+intros h1 a, rw equivalence, split,
+cases h1, exact h1_left a,
+split, cases h1 with h1 h2, rw symmetric,
+intros x y h3, specialize h2 a, rw euclidean at h2, 
+specialize h1 a, rw reflexive at h1,
+specialize h1 x, exact h2 h3 h1,
+rw transitive, intros x y z h2 h3, cases h1 with h1 h4,
+specialize h4 a, rw euclidean at h4, specialize h1 a, 
+rw reflexive at h1, specialize h1 x, have h5 := h4 h2 h1, 
+exact h4 h5 h3
 end
