src/del/semantics/translationfunction.lean
@@ -2,12 +2,12 @@ import del.languageDEL del.semantics.complexitylemmas
 variables {agents : Type}
 
 -- Def 7.20, pg. 186, Translation function t
-@[simp] def translate : formPA agents → formPA agents
-  | (formPA.bot)     := ⊥
-  | (p n)            := p n
-  | (φ & ψ)          := have _, from tr1 φ ψ, have _, from tr2 φ ψ, (translate φ) & (translate ψ)
-  | (φ ⊃ ψ)          := have _, from tr1 φ ψ, have _, from tr2 φ ψ, (translate φ) ⊃ (translate ψ)
-  | (K a φ)          := K a (translate φ)
+@[simp] def translate : formPA agents → form agents
+  | (formPA.bot)     := form.bot
+  | (p n)            := form.var n
+  | (φ & ψ)          := have _, from tr1 φ ψ, have _, from tr2 φ ψ, form.and (translate φ) (translate ψ)
+  | (φ ⊃ ψ)          := have _, from tr1 φ ψ, have _, from tr2 φ ψ, form.impl (translate φ) (translate ψ)
+  | (K a φ)          := form.box a (translate φ)
   | (U φ formPA.bot) := have _, from tr3 φ,     translate (φ ⊃ ⊥)
   | (U φ (p n))      := have _, from tr3 φ,     translate (φ ⊃ (p n))
   | (U φ (ψ & χ))    := have _, from tr5 φ ψ χ, translate ((U φ ψ) & (U φ χ))
