src/del/syntax/syntaxDEL.lean
@@ -8,24 +8,52 @@ variables {agents : Type}
 ---------------------- Proof System ----------------------
 
 -- Define a context
-@[reducible] def ctx (agents: Type) : Type := set (formPA agents)
-notation Γ `un` φ := set.insert φ Γ
+@[reducible] def ctx (agents: Type) : Type := set (form agents)
+instance : has_emptyc (ctx agents) := by apply_instance
+notation Γ `∪` φ := set.insert φ Γ
 
 -- Proof system, pg. 26
-inductive prfPA : ctx agents → formPA agents → Prop 
+inductive prfS5 : ctx agents → form agents → Prop 
+| ax {Γ} {φ} (h : φ ∈ Γ) : prfS5 Γ φ
+| pl1 {Γ} {φ ψ}          : prfS5 Γ (form.impl φ (form.impl ψ φ))
+| pl2 {Γ} {φ ψ χ}        : prfS5 Γ ((φ ⊃ (ψ ⊃ χ)) ⊃ ((φ ⊃ ψ) ⊃ (φ ⊃ χ)))
+| pl3 {Γ} {φ ψ}          : prfS5 Γ (((¬φ) ⊃ (¬ψ)) ⊃ (((¬φ) ⊃ ψ) ⊃ φ))
+| pl4 {Γ} {φ ψ}          : prfS5 Γ (φ ⊃ (ψ ⊃ (φ & ψ)))
+| pl5 {Γ} {φ ψ}          : prfS5 Γ ((φ & ψ) ⊃ φ)
+| pl6 {Γ} {φ ψ}          : prfS5 Γ ((φ & ψ) ⊃ ψ)
+| pl7 {Γ} {φ}            : prfS5 Γ ((¬¬φ) ⊃ φ)
+| pl8 {Γ} {φ ψ}          : prfS5 Γ (((¬φ) ⊃ (¬ψ)) ⊃ (ψ ⊃ φ))
+| kdist {Γ} {φ ψ} {a}    : prfS5 Γ ((K a (φ ⊃ ψ)) ⊃ ((K a φ) ⊃ (K a ψ)))
+| truth {Γ} {φ} {a}      : prfS5 Γ ((K a φ) ⊃ φ)
+| posintro {Γ} {φ} {a}   : prfS5 Γ ((K a φ) ⊃ (K a (K a φ)))
+| negintro {Γ} {φ} {a}   : prfS5 Γ ((¬(K a φ)) ⊃ (K a ¬(K a φ)))
+| mp {Γ} {φ ψ} 
+  (hpq: prfS5 Γ (φ ⊃ ψ)) 
+  (hp : prfS5 Γ φ)       : prfS5 Γ ψ
+| nec {Γ} {φ} {a}
+  (hp: prfS5 Γ φ)        : prfS5 Γ (K a φ)
+
+
+-- Define a context
+@[reducible] def ctxPA (agents: Type) : Type := set (formPA agents)
+--instance : has_emptyc (ctxPA agents) := by apply_instance
+notation Γ `∪` φ := set.insert φ Γ
+
+-- Proof system
+inductive prfPA : ctxPA agents → formPA agents → Prop 
 | ax {Γ} {φ} (h : φ ∈ Γ) : prfPA Γ φ
 | pl1 {Γ} {φ ψ}          : prfPA Γ (φ ⊃ (ψ ⊃ φ))
 | pl2 {Γ} {φ ψ χ}        : prfPA Γ ((φ ⊃ (ψ ⊃ χ)) ⊃ ((φ ⊃ ψ) ⊃ (φ ⊃ χ)))
-| pl3 {Γ} {φ ψ}          : prfPA Γ (((~φ) ⊃ (~ψ)) ⊃ (((~φ) ⊃ ψ) ⊃ φ))
+| pl3 {Γ} {φ ψ}          : prfPA Γ (((¬φ) ⊃ (¬ψ)) ⊃ (((¬φ) ⊃ ψ) ⊃ φ))
 | pl4 {Γ} {φ ψ}          : prfPA Γ (φ ⊃ (ψ ⊃ (φ & ψ)))
 | pl5 {Γ} {φ ψ}          : prfPA Γ ((φ & ψ) ⊃ φ)
 | pl6 {Γ} {φ ψ}          : prfPA Γ ((φ & ψ) ⊃ ψ)
-| pl7 {Γ} {φ}            : prfPA Γ ((~~φ) ⊃ φ)
-| pl8 {Γ} {φ ψ}          : prfPA Γ (((~φ) ⊃ (~ψ)) ⊃ (ψ ⊃ φ))
+| pl7 {Γ} {φ}            : prfPA Γ ((¬¬φ) ⊃ φ)
+| pl8 {Γ} {φ ψ}          : prfPA Γ (((¬φ) ⊃ (¬ψ)) ⊃ (ψ ⊃ φ))
 | kdist {Γ} {φ ψ} {a}    : prfPA Γ ((K a (φ ⊃ ψ)) ⊃ ((K a φ) ⊃ (K a ψ)))
 | truth {Γ} {φ} {a}      : prfPA Γ ((K a φ) ⊃ φ)
 | posintro {Γ} {φ} {a}   : prfPA Γ ((K a φ) ⊃ (K a (K a φ)))
-| negintro {Γ} {φ} {a}   : prfPA Γ ((~(K a φ)) ⊃ (K a ~(K a φ)))
+| negintro {Γ} {φ} {a}   : prfPA Γ ((¬(K a φ)) ⊃ (K a ¬(K a φ)))
 | mp {Γ} {φ ψ} 
   (hpq: prfPA Γ (φ ⊃ ψ)) 
   (hp : prfPA Γ φ)       : prfPA Γ ψ
@@ -33,7 +61,7 @@ inductive prfPA : ctx agents → formPA agents → Prop
   (hp: prfPA Γ φ)        : prfPA Γ (K a φ)
 | atomicbot {Γ} {φ}      : prfPA Γ ((U φ ⊥) ↔ (φ ⊃ ⊥))
 | atomicperm {Γ} {φ} {n} : prfPA Γ ((U φ (p n)) ↔ (φ ⊃ (p n)))
-| announceneg {Γ} {φ ψ}  : prfPA Γ ((U φ (~ψ)) ↔ (φ ⊃ ~(U φ ψ)))
+| announceneg {Γ} {φ ψ}  : prfPA Γ ((U φ (¬ψ)) ↔ (φ ⊃ ¬(U φ ψ)))
 | announceconj {Γ} 
   {φ ψ χ}                : prfPA Γ ((U φ (ψ & χ)) ↔ ((U φ ψ) & (U φ χ)))
 | announceimp {Γ} 
