src/del/announcements.lean
@@ -10,19 +10,19 @@ local attribute [instance] classical.prop_decidable
 
 -- Proposition 4.10, pg. 77
 lemma functional_announce (φ ψ : formPA agents) : 
-  F_valid ((~(U φ (~ψ))) ⊃ (U φ ψ)) equiv_class :=
+  F_validPA ((¬(U φ (¬ψ))) ⊃ (U φ ψ)) equiv_class :=
 begin
-rw F_valid, intros f h v x,
-rw forces, intro h1,
+rw F_validPA, intros f h v x,
+rw forcesPA, intro h1,
 rw forces_update_dual at h1,
 cases h1 with Ph1 h1, intro h, exact h1
 end
 
 -- Proposition 4.11, pg. 77
 lemma partial_announce (φ ψ : formPA agents) : 
-  ¬ (F_valid ~(U φ ~⊥)) equiv_class :=
+  ¬ (F_validPA ¬(U φ ¬⊥)) equiv_class :=
 begin
-rw F_valid, 
+rw F_validPA, 
 push_neg,
 let f : frame agents := { states := nat,
   h := ⟨0⟩,
@@ -37,20 +37,20 @@ exact eq.trans h1 h2,
 let v : nat → f.states → Prop := λ n x, false,
 use v,
 let x : f.states := 42,
-use x, rw forces, rw not_imp,
+use x, rw forcesPA, rw not_imp,
 split, intro h, intro h1, exact h1,
-rw forces, trivial
+rw forcesPA, trivial
 end
 
 -- Proposition 4.12, pg. 77
 lemma public_announce_neg (φ ψ : formPA agents) : 
-  F_valid (U φ (~ψ) ↔ (φ ⊃ ~(U φ ψ))) equiv_class :=
+  F_validPA (U φ (¬ψ) ↔ (φ ⊃ ¬(U φ ψ))) equiv_class :=
 begin
-rw F_valid, intros f h1 v x, split,
+rw F_validPA, intros f h1 v x, split,
 intros h1 h2 h3, specialize h1 h2,
-specialize h3 h2, rw ←not_forces_imp at h1,
+specialize h3 h2, rw ←not_forces_impPA at h1,
 exact absurd h3 h1,
-intros h1, rw forces at h1, rw imp_iff_not_or at h1,
+intros h1, rw forcesPA at h1, rw imp_iff_not_or at h1,
 cases h1,
 intro h2, exact absurd h2 h1_1,
 intros h h1, apply h1_1, intro h2, exact h1
@@ -59,11 +59,11 @@ end
 -- Proposition 4.17, pg. 78
 lemma public_announce_comp (φ ψ χ : formPA agents) (f : frame agents) 
   (v : nat → f.states → Prop) (s : f.states) :
-  forces f v s (U (φ & U φ ψ) χ) ↔ forces f v s (U φ (U ψ χ)) :=
+  forcesPA f v s (U (φ & U φ ψ) χ) ↔ forcesPA f v s (U φ (U ψ χ)) :=
 begin
 split,
 intro h1,
-intro h2,
+intro h2, 
 sorry,
 intro h1,
 intro h2, 
@@ -73,19 +73,19 @@ end
 -- Proposition 4.18, pg. 79
 lemma public_announce_know (φ ψ : formPA agents) (f : frame agents) 
   (v : nat → f.states → Prop) (s : f.states) (a : agents) :
-  forces f v s (U φ (K a ψ)) ↔ forces f v s (φ ⊃ (K a (U φ ψ))) :=
+  forcesPA f v s (U φ (K a ψ)) ↔ forcesPA f v s (φ ⊃ (K a (U φ ψ))) :=
 begin
 split,
 intros h1 h2 t hrel h3,
-rw forces at h1,
+rw forcesPA at h1,
 specialize h1 h2,
-rw forces at h1,
+rw forcesPA at h1,
 specialize h1 ⟨t, h3⟩,
 specialize h1 hrel,
 exact h1,
 intro h1,
 intro h2,
-rw forces,
+rw forcesPA,
 rintro ⟨t, h3⟩,
 intro hrel,
 exact h1 h2 t hrel h3,
@@ -94,14 +94,14 @@ end
 --prop 4.22
 lemma rwVar (φ : formPA agents) (f : frame agents) 
   (v : nat → f.states → Prop) (x : f.states) (n : ℕ) :
-  forces f v x (U φ p n) ↔ forces f v x (φ ⊃ (p n)) :=
+  forcesPA f v x (U φ p n) ↔ forcesPA f v x (φ ⊃ (p n)) :=
 begin
 split, repeat {intros h1 h2, exact h1 h2},
 end
 
 lemma rwAnd (φ ψ χ : formPA agents) (f : frame agents) 
   (v : nat → f.states → Prop) (x : f.states) (n : ℕ) :
-  forces f v x (U φ (ψ & χ)) ↔ forces f v x ((U φ ψ) & (U φ χ)) :=
+  forcesPA f v x (U φ (ψ & χ)) ↔ forcesPA f v x ((U φ ψ) & (U φ χ)) :=
 begin
 split,
 intro h1,
