src/del/semantics/completenessDEL.lean
@@ -1,0 +1,244 @@
+import del.semantics.consistencyDEL del.syntax.soundnessDEL
+import data.list.basic
+local attribute [instance] classical.prop_decidable
+
+open prfS5
+open S5lemma
+variables {agents : Type}
+namespace canonical
+
+
+def canonical [hax : sem_cons (∅ : ctx agents) equiv_class] : frame agents := 
+{ 
+  states := {xΓ : ctx agents // max_ax_consist xΓ},
+  h := begin have h1 := max_ax_exists hax, choose Γ h1 using h1, exact ⟨⟨Γ, h1⟩⟩ end,
+  rel := λ a, λ xΓ yΔ, ∀ φ : form agents, K a φ ∈ xΓ.val → φ ∈ yΔ.val
+}
+
+def val_canonical [hax : sem_cons (∅ : ctx agents) equiv_class] : 
+  nat → canonical.states → Prop := λ n, λ xΓ : canonical.states, (form.var n) ∈ (xΓ.val : ctx agents)
+
+lemma existence (hax : sem_cons (∅ : ctx agents) equiv_class) (xΓ : canonical.states) :
+  ∀ a, ∀ φ : form agents, (¬ K a (¬φ)) ∈ xΓ.val ↔ ∃ yΔ : canonical.states, φ ∈ yΔ.val ∧ canonical.rel a xΓ yΔ :=
+begin
+intros a φ, split,
+intro h1,
+let Γbox : ctx agents := {ψ : form agents | K a ψ ∈ xΓ.val},
+have h1 : ax_consist (Γbox ∪ {φ}), 
+{by_contradiction h2, simp at h2,
+have h3 := five Γbox φ h2,
+cases h3 with L h3, cases h3 with h3 h4,
+have h5 := cut fin_conj_boxn (mp kdist (nec h4)),
+have h6 := exercise1,
+specialize h6 xΓ.2,
+have h7 : ∀ ψ ∈ (list.map (form.box a) L), ψ ∈ xΓ.1, 
+intros ψ h8, simp at *, cases h8 with a h8,
+cases h8 with h8l h8r, specialize h3 a h8l, 
+subst h8r, exact h3,
+specialize h6 h7 h5,
+have h8 := (six xΓ.1 (max_imp_ax xΓ.2)).mp xΓ.2 (K a (¬φ)),
+cases h8 with h8l h8r, simp at *, specialize h8r h6, 
+exact absurd h1 h8r,
+},
+have h2 := lindenbaum (Γbox ∪ {φ}) h1,
+cases h2 with Δ h2, cases h2 with h2 h3,
+let xΔ : canonical.states := ⟨Δ, h2⟩,
+existsi (xΔ : canonical.states),
+have h5 := set.union_subset_iff.mp h3,
+cases h5, split, simp at h5_right, exact h5_right,
+have h3 : ∀ φ : form agents, K a φ ∈ xΓ.val → φ ∈ xΔ.val,
+intros ψ h4, apply h5_left, exact h4,
+exact h3,
+simp at *,
+intros yΔ h1 h2,
+have h3 := h2 φ, 
+by_contradiction h4,
+have h5 := (max_notiff xΓ.1 xΓ.2 (C a φ)).mp h4,
+have h6 := (max_dn xΓ.1 xΓ.2 (K a ¬φ)).mpr h5,
+have h7 := h2 (¬φ), specialize h7 h6,
+simp at *,
+have h8 := (max_notiff yΔ.1 yΔ.2 φ).mpr h7,
+exact absurd h1 h8
+end
+
+lemma truth (hax : sem_cons (∅ : ctx agents) equiv_class) (xΓ : canonical.states) : 
+  ∀ φ : form agents, forces canonical val_canonical xΓ φ ↔ (φ ∈ xΓ.val) :=
+begin
+intro φ, induction φ with n φ ψ ih_φ ih_ψ 
+φ ψ ih_φ ih_ψ φ ih_φ generalizing xΓ,
+split, intro h1, exact false.elim h1,
+intro h1, rw forces, 
+have h2 := xΓ.2,
+rw max_ax_consist at h2, cases h2,
+rw ax_consist at h2_left, specialize h2_left [⊥],
+simp at *, specialize h2_left h1, 
+rw fin_ax_consist at h2_left,
+repeat {rw fin_conj at h2_left},
+exact absurd not_contra h2_left,
+repeat {rw forces, rw val_canonical},
+split, intro h1, cases h1 with h1 h2,
+specialize ih_φ xΓ, cases ih_φ,
+specialize ih_ψ xΓ,
+specialize ih_φ_mp h1, cases ih_ψ,
+specialize ih_ψ_mp h2, 
+exact max_conj_1 xΓ.2 (and.intro ih_φ_mp ih_ψ_mp), 
+intro h1, split,
+specialize ih_φ xΓ, cases ih_φ, 
+apply ih_φ_mpr, exact max_conj_2 xΓ.2 h1,
+specialize ih_ψ xΓ, cases ih_ψ, 
+apply ih_ψ_mpr, exact max_conj_3 xΓ.2 h1,
+split, 
+intro h1, specialize ih_φ xΓ,
+specialize ih_ψ xΓ, cases ih_φ, cases ih_ψ,
+apply max_imp_1 xΓ.2,
+intro h2, specialize ih_φ_mpr h2,
+specialize h1 ih_φ_mpr, exact ih_ψ_mp h1,
+intros h1 h2,
+specialize ih_φ xΓ, cases ih_φ,
+specialize ih_ψ xΓ, cases ih_ψ,
+apply ih_ψ_mpr, specialize ih_φ_mp h2,
+exact max_imp_2 xΓ.2 h1 ih_φ_mp,
+split, 
+rename φ a, rename ih_φ φ,
+intros h1, by_contradiction h2,
+have h4 : C a (¬φ) ∈ xΓ.val → ∃ yΔ : canonical.states, 
+  (¬φ) ∈ yΔ.val ∧ canonical.rel _ xΓ yΔ,
+from (existence hax xΓ a (¬φ)).mp,
+have h5 := max_boxdn xΓ.1 xΓ.2 φ a ((max_notiff xΓ.1 xΓ.2 (K a φ)).mp h2),
+simp at *,
+specialize h4 h5, cases h4 with xΔ h4, cases h4 with h4 h6,
+have h7 := max_notiff xΔ.1 xΔ.2 φ,
+cases h7 with h7l h7r,
+specialize h7r h4, clear h7l h4 h5 h2,
+specialize φ_ih xΔ, specialize h1 xΔ h6,
+cases φ_ih, specialize φ_ih_mp h1,
+exact absurd φ_ih_mp h7r,
+rename φ a, rename ih_φ φ,
+intros h1 xΔ h2,
+have h3 := h2 φ h1,
+specialize φ_ih xΔ, cases φ_ih, 
+apply φ_ih_mpr, exact h3,
+end
+
+lemma comphelper (φ : form agents) (hax : sem_cons (∅ : ctx agents) equiv_class) : 
+  ¬ prfS5 ∅ φ → ax_consist ({¬φ} : ctx agents) :=
+begin
+intro h1, rw ax_consist, intros L h2,
+rw fin_ax_consist, induction L, rw fin_conj, 
+by_contradiction h3,
+exact absurd (mp dne h3) (nprfalse hax), 
+have h4 : (∀ ψ ∈ L_hd::L_tl, ψ = ¬φ) → prfS5 ∅ (¬fin_conj (L_hd::L_tl)) → prfS5 ∅ φ, 
+from fin_conj_repeat hax,
+simp at *, 
+cases h2 with h2 h3,
+specialize h4 h2, intro h6, apply h1, apply h4, 
+exact h3,
+exact h6
+end 
+
+theorem forcesAX (hax : sem_cons (∅ : ctx agents) equiv_class) : 
+  forces_ctx canonical val_canonical (∅ : ctx agents) :=
+begin
+rw forces_ctx,
+intros φ xΓ h1,
+have h2 : prfS5 ∅ (form.impl (¬form.bot) φ), from mp prfS5.pl1 (ax h1),
+have h3 : ∀ ψ ∈ list.nil, ψ ∈ xΓ.val, 
+{intros ψ h3, have h5 := list.ne_nil_of_length_pos (list.length_pos_of_mem h3),
+simp at *, exact false.elim h5},
+have h4 : φ ∈ xΓ.val, from exercise1 xΓ.2 h3 h2,
+exact (truth hax xΓ φ).mpr h4
+end
+
+lemma euclid_dual {a : agents} {φ : form agents} : 
+  prfS5 ∅ ((C a (¬φ) ⊃ K a (C a (¬φ))) ⊃ (C a (K a φ) ⊃ K a φ)) :=
+begin
+simp,
+have h1 : prfS5 ∅ (C a (¬φ) ⊃ K a (C a ¬φ)), from negintro,
+simp at *,
+have h2 : prfS5 ∅ ((¬K a (C a ¬φ)) ⊃ ¬(C a ¬φ)), from contrapos.mpr h1,
+have h3 : prfS5 ∅ ((¬K a (C a ¬φ)) ⊃ (K a φ)), from cut h2 (mp pl6 dual_equiv1),
+have h4 : prfS5 ∅ ((¬K a (C a ¬φ)) ↔ (¬¬C a (¬(C a ¬φ)))),
+  from (mp (mp pl4 (contrapos.mpr (mp pl6 dual_equiv1))) 
+  (contrapos.mpr (mp pl5 dual_equiv1))),
+have h5 : prfS5 ∅ (C a (¬(C a ¬φ)) ⊃ (K a φ)), from cut dni (cut (mp pl6 h4) h3),
+have h6 : prfS5 ∅ ((C a (K a φ)) ⊃ (C a (¬(C a ¬φ)))), 
+  from (contrapos.mpr (mp kdist (nec (contrapos.mpr (mp pl5 dual_equiv1))))),
+exact (mp pl1 (cut h6 h5))
+end
+
+lemma S5_equiv {a : agents} (hax : sem_cons (∅ : ctx agents) equiv_class) : 
+  canonical ∈ (equiv_class : set (frame agents)) :=
+begin
+rw equiv_ref_euclid,
+split,
+rw ref_class, rw set.mem_set_of_eq,
+intro a,
+rw reflexive,
+intros x φ h1,
+have h2 : ∀ a, (∀ ψ ∈ [(K a φ)], ψ ∈ x.1) → prfS5 ∅ (fin_conj [(K a φ)] ⊃ φ) → φ ∈ x.1, 
+  from λ a, exercise1 x.2,
+have h3 : prfS5 ∅ (fin_conj [(K a φ)] ⊃ φ), 
+{repeat {rw fin_conj},
+have h4 : prfS5 ∅ ((K a φ) ⊃ φ), from prfS5.truth,
+exact cut (mp pl5 phi_and_true) h4},
+specialize h2 a, simp at *,
+exact h2 h1 h3,
+rw euclid_class,
+rw set.mem_set_of_eq,
+intro a,
+rw euclidean,
+intros x y z h1 h2 φ h3,
+specialize h2 φ,
+apply h2, clear h2,
+have h2 : prfS5 ∅ (C a (¬φ) ⊃ K a (C a ¬φ)), from negintro,
+have h4 : prfS5 ∅ (C a (K a φ) ⊃ K a φ), 
+  from mp euclid_dual h2,
+have h5 : ∀ a, (∀ ψ ∈ [(C a (K a φ))], ψ ∈ x.1) → 
+  prfS5 ∅ (fin_conj [(C a (K a φ))] ⊃ K a φ) → K a φ ∈ x.1,
+  from λ a, exercise1 x.2, 
+simp at *,
+apply h5,
+by_contradiction h6,
+have h7 : (¬K a (¬K a φ)) ∉ x.1 ↔ (¬(¬K a (¬K a φ))) ∈ x.1, 
+  from max_notiff x.1 x.2 (¬K a (¬K a φ)),
+cases h7, simp at *, specialize h7_mp h6,
+have h8 : (K a (¬K a φ)) ∈ x.1 ↔ (¬¬(K a (¬K a φ))) ∈ x.1, 
+  from max_dn x.1 x.2 (K a (¬K a φ)),
+cases h8, simp at *, specialize h8_mpr h7_mp,
+specialize h1 (¬K a φ) h8_mpr,
+have h9 := (max_notiff y.1 y.2 (K a φ)).mpr h1,
+simp at *, exact absurd h3 h9,
+exact (cut (mp pl5 phi_and_true) h4)
+end
+
+
+theorem completeness (hax : sem_cons (∅ : ctx agents) equiv_class) (φ : form agents) : 
+  global_sem_csq ∅ equiv_class φ → prfS5 ∅ φ :=
+begin
+rw ←not_imp_not, intro h1,
+have h2 : ax_consist {¬φ}, from comphelper φ hax h1,
+have h3 : ∃ Γ', max_ax_consist Γ' ∧ {¬φ} ⊆ Γ', from lindenbaum {¬φ} h2,
+simp at *,
+cases h3 with Γ' h3, cases h3 with h3 h4, 
+rw global_sem_csq, 
+push_neg,
+let f := canonical, 
+use f,
+let v := val_canonical, 
+split,
+exact S5_equiv hax,
+sorry,
+use v,
+let xΓ' : f.states := ⟨Γ', h3⟩,
+split, 
+exact forcesAX hax,
+use xΓ',
+have h5 : forces f v xΓ' (¬φ) ↔ ((¬φ) ∈ xΓ'.val), 
+  from truth hax xΓ' ¬φ,
+cases h5 with h5 h6,
+have h7 : ¬forces f v xΓ' φ ↔ forces f v xΓ' ¬φ, 
+  from not_forces_imp f v xΓ' φ,
+cases h7 with h7 h8, apply h8, apply h6, simp at *, exact h4
+end
+
+end canonical
