src/del/semantics/translationdefs.lean
@@ -7,13 +7,12 @@ variables {agents : Type}
 
 -- Subformulas
 def subformulas : formPA agents → set (formPA agents)
-  | (formPA.bot) := {⊥}
-  | (p n)        := {(p n)}
-  | (~ φ)        := {(~φ)} ∪ (subformulas φ)
-  | (φ & ψ)      := {(φ & ψ)} ∪ (subformulas φ) ∪ (subformulas ψ)
-  | (φ ⊃ ψ)      := {(φ ⊃ ψ)} ∪ (subformulas φ) ∪ (subformulas ψ)
-  | (K a φ)      := {(K a φ)} ∪ (subformulas φ)
-  | (U φ ψ)      := {(U φ ψ)} ∪ (subformulas φ) ∪ (subformulas ψ)
+  | (⊥)       := {⊥}
+  | (p n)     := {(p n)}
+  | (φ & ψ)   := {(φ & ψ)} ∪ (subformulas φ) ∪ (subformulas ψ)
+  | (φ ⊃ ψ)   := {(φ ⊃ ψ)} ∪ (subformulas φ) ∪ (subformulas ψ)
+  | (K a φ)   := {(K a φ)} ∪ (subformulas φ)
+  | (U φ ψ)   := {(U φ ψ)} ∪ (subformulas φ) ∪ (subformulas ψ)
 
 
 -- Def 7.21, pg. 187, Complexity function c
