src/del/semantics/translationlemmas.lean
@@ -1,12 +1,14 @@
 -- Following the textbook "Dynamic Epistemic Logic" by 
 -- Hans van Ditmarsch, Wiebe van der Hoek, and Barteld Kooi
 
-import del.syntax.syntaxDEL del.syntax.syntaxlemmasDEL del.semantics.translationfunction
+import del.syntax.syntaxDEL del.syntax.syntaxlemmasPADEL
+import del.semantics.translationfunction
 variables {agents : Type}
 
 open prfPA
+open PAlemma
 
-lemma iff_iff_imp_iff {Γ : ctx agents} {φ ψ χ θ : formPA agents} : 
+lemma iff_iff_imp_iff {Γ : ctxPA agents} {φ ψ χ θ : formPA agents} : 
   prfPA Γ (φ ↔ χ) → prfPA Γ (ψ ↔ θ) → prfPA Γ ((φ ⊃ ψ) ↔ (χ ⊃ θ)) :=
 begin
 intros h1 h2,
@@ -15,7 +17,7 @@ exact (mp (mp pl4 (imp_switch (cut1 (cut (mp pl6 h1) likemp) (mp pl5 h2))))
 end
 
 
-lemma iff_k_dist {Γ : ctx agents} {φ ψ : formPA agents} {a : agents} :
+lemma iff_k_dist {Γ : ctxPA agents} {φ ψ : formPA agents} {a : agents} :
   prfPA Γ (φ ↔ ψ) → prfPA Γ (K a φ ↔ K a ψ) :=
 begin
 intro h1,
@@ -23,7 +25,7 @@ exact (mp (mp pl4 (mp kdist (nec (mp pl5 h1)))) (mp kdist (nec (mp pl6 h1)))),
 end
 
 
-lemma update_iff1 {Γ : ctx agents} {φ ψ χ : formPA agents} : 
+lemma update_iff1 {Γ : ctxPA agents} {φ ψ χ : formPA agents} : 
   prfPA Γ (φ ↔ χ) → prfPA Γ (U φ ψ ↔ (φ ⊃ ψ)) → prfPA Γ (U φ ψ ↔ (χ ⊃ ψ)) :=
 begin
 intros h1 h2,
@@ -31,10 +33,10 @@ exact (mp (mp pl4 (cut2 (mp pl6 h1) (mp pl5 h2))) (cut (mp hs2 (mp pl5 h1)) (mp 
 end
 
 
-lemma update_iff2 {Γ : ctx agents} {φ ψ χ : formPA agents} : 
-  prfPA Γ ((U φ ψ) ↔ translate (U φ ψ)) → prfPA Γ ((U φ χ) ↔ translate (U φ χ)) → 
+lemma update_iff2 {Γ : ctxPA agents} {φ ψ χ : formPA agents} : 
+  prfPA Γ ((U φ ψ) ↔ to_PA (translate (U φ ψ))) → prfPA Γ ((U φ χ) ↔ to_PA (translate (U φ χ))) → 
   prfPA Γ ((U φ (ψ & χ) ↔ (U φ ψ & U φ χ))) → 
-  prfPA Γ ((U φ (ψ & χ) ↔ translate (U φ ψ) & translate (U φ χ))) :=
+  prfPA Γ ((U φ (ψ & χ) ↔ to_PA (translate (U φ ψ)) & to_PA (translate (U φ χ)))) :=
 begin
 intros h1 h2 h3,
 exact (mp (mp pl4 (cut (mp pl5 h3) (imp_and_and_imp 
@@ -43,12 +45,12 @@ exact (mp (mp pl4 (cut (mp pl5 h3) (imp_and_and_imp
 end
 
 
-lemma update_iff3 {Γ : ctx agents} {φ ψ χ : formPA agents} : 
-  prfPA Γ (U φ ψ ↔ translate (U φ ψ)) →
-  prfPA Γ (U φ χ ↔ translate (U φ χ)) →
+lemma update_iff3 {Γ : ctxPA agents} {φ ψ χ : formPA agents} : 
+  prfPA Γ (U φ ψ ↔ to_PA (translate (U φ ψ))) →
+  prfPA Γ (U φ χ ↔ to_PA (translate (U φ χ))) →
   prfPA Γ (U φ (ψ ⊃ χ) ↔ (U φ ψ ⊃ U φ χ)) → 
   prfPA Γ
-    (U φ (ψ ⊃ χ) ↔ (translate (U φ ψ) ⊃ translate (U φ χ))) :=
+    (U φ (ψ ⊃ χ) ↔ to_PA (translate (U φ ψ)) ⊃ to_PA (translate (U φ χ))) :=
 begin
 intros h1 h2 h3, 
 exact mp (mp pl4 (cut2 (mp pl6 h1) (cut1 (mp pl5 h3) (mp pl5 h2)))) 
@@ -56,10 +58,10 @@ exact mp (mp pl4 (cut2 (mp pl6 h1) (cut1 (mp pl5 h3) (mp pl5 h2))))
 end
 
 
-lemma update_iff4 {Γ : ctx agents} {φ ψ : formPA agents} {a : agents} : 
+lemma update_iff4 {Γ : ctxPA agents} {φ ψ : formPA agents} {a : agents} : 
   prfPA Γ ((U φ (K a ψ) ↔ (φ ⊃ K a (U φ ψ)))) → 
-  prfPA Γ ((φ ⊃ K a (U φ ψ)) ↔ translate (φ ⊃ K a (U φ ψ))) → 
-  prfPA Γ (U φ (K a ψ) ↔ (translate φ ⊃ K a (translate (U φ ψ)))) :=
+  prfPA Γ ((φ ⊃ K a (U φ ψ)) ↔ to_PA (translate (φ ⊃ K a (U φ ψ)))) → 
+  prfPA Γ (U φ (K a ψ) ↔ (to_PA (translate φ) ⊃ K a (to_PA (translate (U φ ψ))))) :=
 begin
 simp at *,
 intros h1 h2, 
@@ -67,10 +69,10 @@ exact mp (mp pl4 (cut (mp pl5 h1) (mp pl5 h2))) (cut (mp pl6 h2) (mp pl6 h1))
 end
 
 
-lemma update_iff5 {Γ : ctx agents} {φ ψ χ : formPA agents} : 
+lemma update_iff5 {Γ : ctxPA agents} {φ ψ χ : formPA agents} : 
   prfPA Γ ((U φ (U ψ χ)) ↔ (U (φ & U φ ψ) χ)) → 
-  prfPA Γ ((U (φ & U φ ψ) χ) ↔ translate (U (φ & U φ ψ) χ)) → 
-  prfPA Γ ((U φ (U ψ χ)) ↔ translate (U (φ & U φ ψ) χ)) :=
+  prfPA Γ ((U (φ & U φ ψ) χ) ↔ to_PA (translate (U (φ & U φ ψ) χ))) → 
+  prfPA Γ ((U φ (U ψ χ)) ↔ to_PA (translate (U (φ & U φ ψ) χ))) :=
 begin
 simp at *,
 intros h1 h2,
