src/del/syntax/syntaxlemmasDEL.lean
@@ -3,29 +3,30 @@
 
 import del.languageDEL del.syntax.syntaxDEL data.set.basic
 
-open prfPA
+open prfS5
 local attribute [instance] classical.prop_decidable
 variables {agents : Type}
 
 
 ---------------------- Helper Lemmas ----------------------
 
+namespace S5lemma
 
-lemma iden {Γ : ctx agents} {φ : formPA agents} :
-  prfPA Γ (φ ⊃ φ) :=
+lemma iden {Γ : ctx agents} {φ : form agents} :
+  prfS5 Γ (φ ⊃ φ) :=
 begin
 exact mp (mp (@pl2 _ _ φ (φ ⊃ φ) φ) pl1) pl1
 end
 
-lemma prtrue {Γ : ctx agents} : prfPA Γ ~⊥ :=
+lemma prtrue {Γ : ctx agents} : prfS5 Γ ¬⊥ :=
 begin
 exact iden
 end
 
-lemma weak {Γ : ctx agents} {φ ψ : formPA agents} :
-  prfPA Γ φ → prfPA (Γ ∪ ψ) φ :=
+lemma weak {Γ : ctx agents} {φ ψ : form agents} :
+  prfS5 Γ φ → prfS5 (Γ ∪ ψ) φ :=
 begin
-  intro h, dsimp,
+  intro h,
   induction h,
   { apply ax,
     exact (set.mem_insert_of_mem _ h_h) },
@@ -44,19 +45,12 @@ begin
   { apply mp,
     { exact h_ih_hpq },
     { exact h_ih_hp } },
-  { exact nec h_ih },
-  { exact atomicbot },
-  { exact atomicperm },
-  { exact announceneg },
-  { exact announceconj },
-  { exact announceimp },
-  { exact announceknow },
-  { exact announcecomp }
+  { exact nec h_ih }
 end
 
 
-lemma pr {Γ : ctx agents} {φ : formPA agents} :
-  prfPA (Γ ∪ φ) φ :=
+lemma pr {Γ : ctx agents} {φ : form agents} :
+  prfS5 (Γ ∪ φ) φ :=
 begin
 apply ax;
 apply or.intro_left;
@@ -64,120 +58,120 @@ simp
 end
 
 
-lemma cut {Γ : ctx agents} {φ ψ χ : formPA agents} :
-  prfPA Γ (φ ⊃ ψ) → prfPA Γ (ψ ⊃ χ) → prfPA Γ (φ ⊃ χ) :=
+lemma cut {Γ : ctx agents} {φ ψ χ : form agents} :
+  prfS5 Γ (φ ⊃ ψ) → prfS5 Γ (ψ ⊃ χ) → prfS5 Γ (φ ⊃ χ) :=
 begin
 intros h1 h2,
 exact mp (mp pl2 (mp pl1 h2)) h1
 end
 
 
-lemma conv_deduction {Γ : ctx agents} {φ ψ : formPA agents} :
-  prfPA Γ (φ ⊃ ψ) → prfPA (Γ ∪ φ) ψ :=
+lemma conv_deduction {Γ : ctx agents} {φ ψ : form agents} :
+  prfS5 Γ (φ ⊃ ψ) → prfS5 (Γ ∪ φ) ψ :=
 begin
 intro h, 
 exact mp (weak h) pr 
 end
 
 
-lemma hs1 {Γ : ctx agents} {φ ψ χ : formPA agents} :
-  prfPA Γ ((ψ ⊃ χ) ⊃ ((φ ⊃ ψ) ⊃ (φ ⊃ χ))) :=
+lemma hs1 {Γ : ctx agents} {φ ψ χ : form agents} :
+  prfS5 Γ ((ψ ⊃ χ) ⊃ ((φ ⊃ ψ) ⊃ (φ ⊃ χ))) :=
 begin
 exact (mp (mp pl2 (mp pl1 pl2)) pl1)
 end
 
 
-lemma likemp {Γ : ctx agents} {φ ψ : formPA agents} : 
-  prfPA Γ (φ ⊃ ((φ ⊃ ψ) ⊃ ψ)) :=
+lemma likemp {Γ : ctx agents} {φ ψ : form agents} : 
+  prfS5 Γ (φ ⊃ ((φ ⊃ ψ) ⊃ ψ)) :=
 begin
 exact (mp (mp hs1 (mp pl2 iden)) pl1)
 end
 
 
-lemma dne {Γ : ctx agents} {φ : formPA agents} :
-prfPA Γ ((~~φ) ⊃ φ) :=
+lemma dne {Γ : ctx agents} {φ : form agents} :
+prfS5 Γ ((¬¬φ) ⊃ φ) :=
 begin
-have h1 : prfPA Γ (φ ⊃ (φ ⊃ φ)), from pl1,
-have h2 : prfPA Γ (((~~(φ ⊃ (φ ⊃ φ))) ⊃ (~~φ)) ⊃ ((~φ) ⊃ ~(φ ⊃ (φ ⊃ φ)))), from pl8,
-have h3 : prfPA Γ (((~φ) ⊃ ~(φ ⊃ (φ ⊃ φ))) ⊃ ((φ ⊃ (φ ⊃ φ)) ⊃ φ)), from pl8,
-have h4 : prfPA Γ (((~~(φ ⊃ (φ ⊃ φ))) ⊃ (~~φ)) ⊃ ((φ ⊃ (φ ⊃ φ)) ⊃ φ)), from cut h2 h3,
-have h5 : prfPA Γ ((~~φ) ⊃ ((~~(φ ⊃ (φ ⊃ φ))) ⊃ (~~φ))), from pl1,
-have h6 : prfPA Γ ((~~φ) ⊃ ((φ ⊃ (φ ⊃ φ)) ⊃ φ)), from cut h5 h4,
-have h7 : prfPA Γ ((φ ⊃ (φ ⊃ φ)) ⊃ (((φ ⊃ (φ ⊃ φ)) ⊃ φ) ⊃ φ)), from likemp,
-have h8 : prfPA Γ (((φ ⊃ (φ ⊃ φ)) ⊃ φ) ⊃ φ), from mp h7 h1,
-have h9 : prfPA Γ ((~~φ) ⊃ φ), from cut h6 h8,
+have h1 : prfS5 Γ (φ ⊃ (φ ⊃ φ)), from pl1,
+have h2 : prfS5 Γ (((¬¬(φ ⊃ (φ ⊃ φ))) ⊃ (¬¬φ)) ⊃ ((¬φ) ⊃ ¬(φ ⊃ (φ ⊃ φ)))), from pl8,
+have h3 : prfS5 Γ (((¬φ) ⊃ ¬(φ ⊃ (φ ⊃ φ))) ⊃ ((φ ⊃ (φ ⊃ φ)) ⊃ φ)), from pl8,
+have h4 : prfS5 Γ (((¬¬(φ ⊃ (φ ⊃ φ))) ⊃ (¬¬φ)) ⊃ ((φ ⊃ (φ ⊃ φ)) ⊃ φ)), from cut h2 h3,
+have h5 : prfS5 Γ ((¬¬φ) ⊃ ((¬¬(φ ⊃ (φ ⊃ φ))) ⊃ (¬¬φ))), from pl1,
+have h6 : prfS5 Γ ((¬¬φ) ⊃ ((φ ⊃ (φ ⊃ φ)) ⊃ φ)), from cut h5 h4,
+have h7 : prfS5 Γ ((φ ⊃ (φ ⊃ φ)) ⊃ (((φ ⊃ (φ ⊃ φ)) ⊃ φ) ⊃ φ)), from likemp,
+have h8 : prfS5 Γ (((φ ⊃ (φ ⊃ φ)) ⊃ φ) ⊃ φ), from mp h7 h1,
+have h9 : prfS5 Γ ((¬¬φ) ⊃ φ), from cut h6 h8,
 exact h9
 end
 
 
-lemma dni {Γ : ctx agents} {φ : formPA agents} : prfPA Γ (φ ⊃ ~~φ) :=
+lemma dni {Γ : ctx agents} {φ : form agents} : prfS5 Γ (φ ⊃ ¬¬φ) :=
 begin
-have h1 : prfPA Γ ((~~(~φ)) ⊃ (~φ)), from dne,
+have h1 : prfS5 Γ ((¬¬(¬φ)) ⊃ (¬φ)), from dne,
 exact mp pl8 h1
 end
 
 
-lemma imp_if_imp_imp {Γ : ctx agents} {φ ψ χ : formPA agents} : prfPA Γ (φ ⊃ χ) → prfPA Γ (φ ⊃ (ψ ⊃ χ)) :=
+lemma imp_if_imp_imp {Γ : ctx agents} {φ ψ χ : form agents} : prfS5 Γ (φ ⊃ χ) → prfS5 Γ (φ ⊃ (ψ ⊃ χ)) :=
 begin
 intro h1,
 exact mp (mp pl2 (mp pl1 pl1)) h1
 end
 
 
-lemma cut1 {Γ : ctx agents} {φ ψ χ θ : formPA agents} :
-  prfPA Γ (θ ⊃ (φ ⊃ ψ)) → prfPA Γ (ψ ⊃ χ) → prfPA Γ (θ ⊃ (φ ⊃ χ)) :=
+lemma cut1 {Γ : ctx agents} {φ ψ χ θ : form agents} :
+  prfS5 Γ (θ ⊃ (φ ⊃ ψ)) → prfS5 Γ (ψ ⊃ χ) → prfS5 Γ (θ ⊃ (φ ⊃ χ)) :=
 begin
 intros h1 h2,
-have h3 : prfPA Γ (φ ⊃ ψ) → prfPA Γ (ψ ⊃ χ) → prfPA Γ (φ ⊃ χ), from cut,
-have h4 : prfPA Γ (θ ⊃ (φ ⊃ ψ)) → prfPA Γ ((φ ⊃ ψ) ⊃ (φ ⊃ χ)) → prfPA Γ (θ ⊃ (φ ⊃ χ)), from cut,
+have h3 : prfS5 Γ (φ ⊃ ψ) → prfS5 Γ (ψ ⊃ χ) → prfS5 Γ (φ ⊃ χ), from cut,
+have h4 : prfS5 Γ (θ ⊃ (φ ⊃ ψ)) → prfS5 Γ ((φ ⊃ ψ) ⊃ (φ ⊃ χ)) → prfS5 Γ (θ ⊃ (φ ⊃ χ)), from cut,
 specialize h4 h1,
-have h5 : prfPA Γ ((φ ⊃ ψ) ⊃ (φ ⊃ χ)), from mp pl2 (mp pl1 h2),
+have h5 : prfS5 Γ ((φ ⊃ ψ) ⊃ (φ ⊃ χ)), from mp pl2 (mp pl1 h2),
 specialize h4 h5,
 exact h4
 end
 
 
-lemma imp_switch {Γ : ctx agents} {φ ψ χ : formPA agents} : prfPA Γ (φ ⊃ (ψ ⊃ χ)) → prfPA Γ (ψ ⊃ (φ ⊃ χ)) :=
+lemma imp_switch {Γ : ctx agents} {φ ψ χ : form agents} : prfS5 Γ (φ ⊃ (ψ ⊃ χ)) → prfS5 Γ (ψ ⊃ (φ ⊃ χ)) :=
 begin
 intro h1,
-have h2 : prfPA Γ (ψ ⊃ ((φ ⊃ ψ) ⊃ (φ ⊃ χ))), from mp pl1 (mp pl2 h1),
-have h3 : prfPA Γ ((ψ ⊃ (φ ⊃ ψ)) ⊃ (ψ ⊃ (φ ⊃ χ))), from mp pl2 h2,
+have h2 : prfS5 Γ (ψ ⊃ ((φ ⊃ ψ) ⊃ (φ ⊃ χ))), from mp pl1 (mp pl2 h1),
+have h3 : prfS5 Γ ((ψ ⊃ (φ ⊃ ψ)) ⊃ (ψ ⊃ (φ ⊃ χ))), from mp pl2 h2,
 exact mp h3 pl1
 end
 
 
-lemma l2 {Γ : ctx agents} {φ ψ χ : formPA agents} : prfPA Γ ((φ ⊃ (ψ ⊃ χ)) ⊃ (ψ ⊃ (φ ⊃ χ))) :=
+lemma l2 {Γ : ctx agents} {φ ψ χ : form agents} : prfS5 Γ ((φ ⊃ (ψ ⊃ χ)) ⊃ (ψ ⊃ (φ ⊃ χ))) :=
 begin
 exact (mp (mp pl2 (cut pl2 hs1)) (mp pl1 pl1))
 end
 
 
-lemma hs2 {Γ : ctx agents} {φ ψ χ : formPA agents} :
-  prfPA Γ ((φ ⊃ ψ) ⊃ ((ψ ⊃ χ) ⊃ (φ ⊃ χ))) :=
+lemma hs2 {Γ : ctx agents} {φ ψ χ : form agents} :
+  prfS5 Γ ((φ ⊃ ψ) ⊃ ((ψ ⊃ χ) ⊃ (φ ⊃ χ))) :=
 begin
 exact (mp l2 hs1)
 end
 
 
-lemma cut2 {Γ : ctx agents} {φ ψ χ θ : formPA agents} :
-  prfPA Γ (φ ⊃ ψ) → prfPA Γ (θ ⊃ (ψ ⊃ χ)) → prfPA Γ (θ ⊃ (φ ⊃ χ)) :=
+lemma cut2 {Γ : ctx agents} {φ ψ χ θ : form agents} :
+  prfS5 Γ (φ ⊃ ψ) → prfS5 Γ (θ ⊃ (ψ ⊃ χ)) → prfS5 Γ (θ ⊃ (φ ⊃ χ)) :=
 begin
 intros h1 h2,
 exact imp_switch (cut h1 (imp_switch h2))
 end
 
 
-lemma double_imp {Γ : ctx agents} {φ ψ : formPA agents} :
-  prfPA Γ ((φ ⊃ (φ ⊃ ψ)) ⊃ (φ ⊃ ψ)) :=
+lemma double_imp {Γ : ctx agents} {φ ψ : form agents} :
+  prfS5 Γ ((φ ⊃ (φ ⊃ ψ)) ⊃ (φ ⊃ ψ)) :=
 begin
-have h1 : prfPA Γ ((φ ⊃ ψ) ⊃ (φ ⊃ ψ)) → prfPA Γ (φ ⊃ ((φ ⊃ ψ) ⊃ ψ)), from imp_switch,
+have h1 : prfS5 Γ ((φ ⊃ ψ) ⊃ (φ ⊃ ψ)) → prfS5 Γ (φ ⊃ ((φ ⊃ ψ) ⊃ ψ)), from imp_switch,
 specialize h1 iden,
 exact mp pl2 h1
 end
 
 
-lemma imp_imp_iff_imp {Γ : ctx agents} {θ φ ψ : formPA agents} : 
-  prfPA Γ (θ ⊃ (φ ⊃ (φ ⊃ ψ))) ↔ prfPA Γ (θ ⊃ (φ ⊃ ψ)) :=
+lemma imp_imp_iff_imp {Γ : ctx agents} {θ φ ψ : form agents} : 
+  prfS5 Γ (θ ⊃ (φ ⊃ (φ ⊃ ψ))) ↔ prfS5 Γ (θ ⊃ (φ ⊃ ψ)) :=
 begin
 split,
 {intro h1,
@@ -187,24 +181,24 @@ exact cut h1 pl1}
 end
 
 
-lemma imp_shift {Γ : ctx agents} {θ φ ψ χ : formPA agents} : 
-  prfPA Γ (θ ⊃ (φ ⊃ (ψ ⊃ χ))) ↔ prfPA Γ (θ ⊃ (ψ ⊃ (φ ⊃ χ))) :=
+lemma imp_shift {Γ : ctx agents} {θ φ ψ χ : form agents} : 
+  prfS5 Γ (θ ⊃ (φ ⊃ (ψ ⊃ χ))) ↔ prfS5 Γ (θ ⊃ (ψ ⊃ (φ ⊃ χ))) :=
 begin
 split,
 repeat {intro h1, exact cut h1 (cut2 pl1 pl2)}
 end
 
 
-lemma left_and_imp {Γ : ctx agents} {φ ψ χ : formPA agents} :
-  prfPA Γ (ψ ⊃ ((φ & ψ) ⊃ χ)) → prfPA Γ ((φ & ψ) ⊃ χ) :=
+lemma left_and_imp {Γ : ctx agents} {φ ψ χ : form agents} :
+  prfS5 Γ (ψ ⊃ ((φ & ψ) ⊃ χ)) → prfS5 Γ ((φ & ψ) ⊃ χ) :=
 begin
 intro h1,
 exact mp double_imp (cut pl6 h1)
 end
 
 
-lemma and_right_imp {Γ : ctx agents} {φ ψ χ : formPA agents} : 
-  prfPA Γ ((φ & ψ) ⊃ χ) ↔ prfPA Γ (ψ ⊃ (φ ⊃ χ)) :=
+lemma and_right_imp {Γ : ctx agents} {φ ψ χ : form agents} : 
+  prfS5 Γ ((φ & ψ) ⊃ χ) ↔ prfS5 Γ (ψ ⊃ (φ ⊃ χ)) :=
 begin
 split, 
 {intro h1,
@@ -214,7 +208,7 @@ exact left_and_imp (cut2 pl5 h1)
 end
 
 
-lemma not_and_subst {φ ψ χ : formPA agents} {Γ : ctx agents} : prfPA Γ (φ ↔ ψ) → (prfPA Γ ~(χ & φ) ↔ prfPA Γ ~(χ & ψ)) :=
+lemma not_and_subst {φ ψ χ : form agents} {Γ : ctx agents} : prfS5 Γ (φ ↔ ψ) → (prfS5 Γ ¬(χ & φ) ↔ prfS5 Γ ¬(χ & ψ)) :=
 begin
 intro h1, split, 
 {intro h2,
@@ -224,36 +218,36 @@ exact mp (mp pl3 (mp pl1 h2)) (cut dne (mp double_imp (cut2 (cut pl6 (mp pl5 h1)
 end
 
 
-lemma not_contra {Γ : ctx agents} {φ : formPA agents} : 
-  prfPA Γ ~(φ & ~φ) :=
+lemma not_contra {Γ : ctx agents} {φ : form agents} : 
+  prfS5 Γ ¬(φ & ¬φ) :=
 begin
 exact mp (mp pl3 (cut dne pl6)) (cut dne pl5)
 end
 
 
-lemma phi_and_true {Γ : ctx agents} {φ : formPA agents} : prfPA Γ ((φ&(~⊥)) ↔ φ) :=
+lemma phi_and_true {Γ : ctx agents} {φ : form agents} : prfS5 Γ ((φ&(¬⊥)) ↔ φ) :=
 begin
 exact (mp (mp pl4 pl5) (mp (imp_switch pl4) prtrue))
 end
 
 
-lemma imp_and_and_imp {Γ : ctx agents} {φ ψ χ θ : formPA agents} : 
-  prfPA Γ (((φ ⊃ ψ) & (χ ⊃ θ))) → prfPA Γ (((φ & χ) ⊃ (ψ & θ))) :=
+lemma imp_and_and_imp {Γ : ctx agents} {φ ψ χ θ : form agents} : 
+  prfS5 Γ (((φ ⊃ ψ) & (χ ⊃ θ))) → prfS5 Γ (((φ & χ) ⊃ (ψ & θ))) :=
 begin
 intro h,
 exact (mp double_imp (cut (cut pl5 (mp pl5 h)) (cut2 (cut pl6 (mp pl6 h)) pl4)))
 end
 
 
-lemma not_contra_equiv_true {Γ : ctx agents} {φ : formPA agents} : 
-  prfPA Γ (~(φ & ~φ) ↔ ~⊥) :=
+lemma not_contra_equiv_true {Γ : ctx agents} {φ : form agents} : 
+  prfS5 Γ (¬(φ & ¬φ) ↔ ¬⊥) :=
 begin
 exact (mp (mp pl4 (mp pl1 prtrue)) (mp pl1 not_contra))
 end
 
 
-lemma contrapos {Γ : ctx agents} {φ ψ : formPA agents} :
-  prfPA Γ ((~ψ) ⊃ (~φ)) ↔ prfPA Γ (φ ⊃ ψ) :=
+lemma contrapos {Γ : ctx agents} {φ ψ : form agents} :
+  prfS5 Γ ((¬ψ) ⊃ (¬φ)) ↔ prfS5 Γ (φ ⊃ ψ) :=
 begin
 split,
 intro h1,
@@ -263,35 +257,35 @@ exact mp (cut (cut (mp hs1 dni) (mp hs2 dne)) pl8) h1,
 end
 
 
-lemma iff_not {Γ : ctx agents} {φ ψ : formPA agents} :
-  prfPA Γ (φ ↔ ψ) → prfPA Γ (~ψ ↔ ~φ) :=
+lemma iff_not {Γ : ctx agents} {φ ψ : form agents} :
+  prfS5 Γ (φ ↔ ψ) → prfS5 Γ (¬ψ ↔ ¬φ) :=
 begin
 intro h1,
-have h2 : prfPA Γ (φ ⊃ ψ), from mp pl5 h1,
-have h3 : prfPA Γ (ψ ⊃ φ), from mp pl6 h1,
+have h2 : prfS5 Γ (φ ⊃ ψ), from mp pl5 h1,
+have h3 : prfS5 Γ (ψ ⊃ φ), from mp pl6 h1,
 rw ←contrapos at h2,
 rw ←contrapos at h3,
 exact (mp (mp pl4 h2) h3)
 end
 
 
-lemma contra_equiv_false {Γ : ctx agents} {φ : formPA agents} : 
-  prfPA Γ ((φ & ~φ) ↔ ⊥) :=
+lemma contra_equiv_false {Γ : ctx agents} {φ : form agents} : 
+  prfS5 Γ ((φ & ¬φ) ↔ ⊥) :=
 begin
-have h1 : prfPA Γ (~~⊥ ↔ ~~(φ & ~φ)), from iff_not not_contra_equiv_true,
+have h1 : prfS5 Γ (¬¬⊥ ↔ ¬¬(φ & ¬φ)), from iff_not not_contra_equiv_true,
 exact (mp (mp pl4 (cut dni (cut (mp pl6 h1) dne))) (cut dni (cut (mp pl5 h1) dne)))
 end
 
 
-lemma and_switch {Γ : ctx agents} {φ ψ : formPA agents} : prfPA Γ ((φ & ψ) ↔ (ψ & φ)) :=
+lemma and_switch {Γ : ctx agents} {φ ψ : form agents} : prfS5 Γ ((φ & ψ) ↔ (ψ & φ)) :=
 begin
 exact (mp (mp pl4 (mp double_imp (cut pl5 (imp_switch (cut pl6 pl4))))) 
 (mp double_imp (cut pl5 (imp_switch (cut pl6 pl4)))))
 end
 
 
-lemma imp_and_imp {Γ : ctx agents} {φ ψ χ : formPA agents} : 
-  prfPA Γ (φ ⊃ ψ) → prfPA Γ  ((χ & φ) ⊃ (χ & ψ)) :=
+lemma imp_and_imp {Γ : ctx agents} {φ ψ χ : form agents} : 
+  prfS5 Γ (φ ⊃ ψ) → prfS5 Γ  ((χ & φ) ⊃ (χ & ψ)) :=
 begin
 intros h1,
 have h2 := imp_and_and_imp,
@@ -299,15 +293,15 @@ specialize h2 (mp (mp pl4 iden) h1), exact h2
 end
 
 
-lemma iff_iff_and_iff {Γ : ctx agents} {φ ψ χ θ : formPA agents} : 
-  prfPA Γ (φ ↔ χ) → prfPA Γ (ψ ↔ θ) → prfPA Γ ((φ & ψ) ↔ (χ & θ)) := 
+lemma iff_iff_and_iff {Γ : ctx agents} {φ ψ χ θ : form agents} : 
+  prfS5 Γ (φ ↔ χ) → prfS5 Γ (ψ ↔ θ) → prfS5 Γ ((φ & ψ) ↔ (χ & θ)) := 
 begin
 intros h1 h2,
 exact mp (mp pl4 (imp_and_and_imp (mp (mp pl4 (mp pl5 h1)) (mp pl5 h2)))) 
   (imp_and_and_imp (mp (mp pl4 (mp pl6 h1)) (mp pl6 h2)))
 end
 
-lemma and_commute {Γ : ctx agents} {φ ψ χ : formPA agents} : prfPA Γ (((φ & ψ) & χ) ↔ (φ & (ψ & χ))) :=
+lemma and_commute {Γ : ctx agents} {φ ψ χ : form agents} : prfS5 Γ (((φ & ψ) & χ) ↔ (φ & (ψ & χ))) :=
 begin
 exact mp (mp pl4 (mp double_imp (imp_imp_iff_imp.mp 
   (cut (cut pl5 pl6) (cut2 pl6 (cut1 pl4 (imp_switch (cut (cut pl5 pl5) pl4)))))))) 
@@ -315,8 +309,8 @@ exact mp (mp pl4 (mp double_imp (imp_imp_iff_imp.mp
   (imp_switch (cut pl5 (cut1 pl4 (cut2 (cut pl6 pl6) pl4)))))))
 end
 
-lemma demorgans {Γ : ctx agents} {φ ψ : formPA agents} : 
-  prfPA Γ (~(φ & ψ)) ↔ prfPA Γ (φ ⊃ ~ψ) :=
+lemma demorgans {Γ : ctx agents} {φ ψ : form agents} : 
+  prfS5 Γ (¬(φ & ψ)) ↔ prfS5 Γ (φ ⊃ ¬ψ) :=
 begin
 split,
 intro h1,
@@ -325,29 +319,25 @@ intro h1,
 exact (mp (contrapos.mpr (mp pl5 and_switch)) (and_right_imp.mpr h1))
 end
 
-lemma explosion {Γ : ctx agents} {ψ : formPA agents} : prfPA Γ (⊥ ⊃ ψ) :=
+lemma explosion {Γ : ctx agents} {ψ : form agents} : prfS5 Γ (⊥ ⊃ ψ) :=
 begin
 apply contrapos.mp, exact (mp pl1 iden)
 end
 
-lemma exfalso {Γ : ctx agents} {φ ψ : formPA agents} : prfPA Γ ((φ & ~φ) ⊃ ψ) :=
+lemma exfalso {Γ : ctx agents} {φ ψ : form agents} : prfS5 Γ ((φ & ¬φ) ⊃ ψ) :=
 begin
 exact cut not_contra explosion
 end
 
-lemma box_dn {Γ : ctx agents} {φ : formPA agents} {a : agents}  : prfPA Γ ((~K a φ) ↔ ~(K a (~~φ))) :=
+lemma box_dn {Γ : ctx agents} {φ : form agents} {a : agents}  : prfS5 Γ ((¬K a φ) ↔ ¬(K a (¬¬φ))) :=
 begin
 exact mp (mp pl4 (contrapos.mpr (mp kdist (nec dne)))) (contrapos.mpr (mp kdist (nec dni)))
 end
 
-lemma dual_equiv1 {Γ : ctx agents} {φ : formPA agents} {a : agents} : prfPA Γ ((K a φ) ↔ (~(~K a ~(~φ)))) :=
+lemma dual_equiv1 {Γ : ctx agents} {φ : form agents} {a : agents} : prfS5 Γ ((K a φ) ↔ (¬(¬K a ¬(¬φ)))) :=
 begin
 exact mp (mp pl4 (cut (contrapos.mp (mp pl6 box_dn)) dni)) 
   (cut dne (contrapos.mp (mp pl5 box_dn)))
 end
 
--- lemma dual_equiv2 {Γ : ctx agents} {φ : formPA agents} {a : agents} : prfPA Γ ((~(K a ~ φ)) ↔ (~ K a ~ φ)) :=
--- begin
--- exact mp (mp pl4 iden) iden,
--- end
-
+end S5lemma
