src/del/syntax/syntaxlemmasPADEL.lean
@@ -1,0 +1,350 @@
+-- Following the textbook "Dynamic Epistemic Logic" by 
+-- Hans van Ditmarsch, Wiebe van der Hoek, and Barteld Kooi
+
+import del.languageDEL del.syntax.syntaxDEL data.set.basic
+
+open prfPA
+local attribute [instance] classical.prop_decidable
+variables {agents : Type}
+
+
+---------------------- Helper Lemmas ----------------------
+
+namespace PAlemma
+
+lemma iden {Γ : ctxPA agents} {φ : formPA agents} :
+  prfPA Γ (φ ⊃ φ) :=
+begin
+exact mp (mp (@pl2 _ _ φ (φ ⊃ φ) φ) pl1) pl1
+end
+
+lemma prtrue {Γ : ctxPA agents} : prfPA Γ ¬⊥ :=
+begin
+exact iden
+end
+
+lemma weak {Γ : ctxPA agents} {φ ψ : formPA agents} :
+  prfPA Γ φ → prfPA (Γ ∪ ψ) φ :=
+begin
+  intro h,
+  induction h,
+  { apply ax,
+    exact (set.mem_insert_of_mem _ h_h) },
+  { exact pl1 },
+  { exact pl2 },
+  { exact pl3 },
+  { exact pl4 },
+  { exact pl5 },
+  { exact pl6 },
+  { exact pl7 },
+  { exact pl8 },
+  { exact kdist },
+  { exact truth },
+  { exact posintro },
+  { exact negintro },
+  { apply mp,
+    { exact h_ih_hpq },
+    { exact h_ih_hp } },
+  { exact nec h_ih },
+  { exact atomicbot },
+  { exact atomicperm },
+  { exact announceneg },
+  { exact announceconj },
+  { exact announceimp },
+  { exact announceknow },
+  { exact announcecomp }
+end
+
+
+lemma pr {Γ : ctxPA agents} {φ : formPA agents} :
+  prfPA (Γ ∪ φ) φ :=
+begin
+apply ax;
+apply or.intro_left;
+simp
+end
+
+
+lemma cut {Γ : ctxPA agents} {φ ψ χ : formPA agents} :
+  prfPA Γ (φ ⊃ ψ) → prfPA Γ (ψ ⊃ χ) → prfPA Γ (φ ⊃ χ) :=
+begin
+intros h1 h2,
+exact mp (mp pl2 (mp pl1 h2)) h1
+end
+
+
+lemma conv_deduction {Γ : ctxPA agents} {φ ψ : formPA agents} :
+  prfPA Γ (φ ⊃ ψ) → prfPA (Γ ∪ φ) ψ :=
+begin
+intro h, 
+exact mp (weak h) pr 
+end
+
+
+lemma hs1 {Γ : ctxPA agents} {φ ψ χ : formPA agents} :
+  prfPA Γ ((ψ ⊃ χ) ⊃ ((φ ⊃ ψ) ⊃ (φ ⊃ χ))) :=
+begin
+exact (mp (mp pl2 (mp pl1 pl2)) pl1)
+end
+
+
+lemma likemp {Γ : ctxPA agents} {φ ψ : formPA agents} : 
+  prfPA Γ (φ ⊃ ((φ ⊃ ψ) ⊃ ψ)) :=
+begin
+exact (mp (mp hs1 (mp pl2 iden)) pl1)
+end
+
+
+lemma dne {Γ : ctxPA agents} {φ : formPA agents} :
+prfPA Γ ((¬¬φ) ⊃ φ) :=
+begin
+have h1 : prfPA Γ (φ ⊃ (φ ⊃ φ)), from pl1,
+have h2 : prfPA Γ (((¬¬(φ ⊃ (φ ⊃ φ))) ⊃ (¬¬φ)) ⊃ ((¬φ) ⊃ ¬(φ ⊃ (φ ⊃ φ)))), from pl8,
+have h3 : prfPA Γ (((¬φ) ⊃ ¬(φ ⊃ (φ ⊃ φ))) ⊃ ((φ ⊃ (φ ⊃ φ)) ⊃ φ)), from pl8,
+have h4 : prfPA Γ (((¬¬(φ ⊃ (φ ⊃ φ))) ⊃ (¬¬φ)) ⊃ ((φ ⊃ (φ ⊃ φ)) ⊃ φ)), from cut h2 h3,
+have h5 : prfPA Γ ((¬¬φ) ⊃ ((¬¬(φ ⊃ (φ ⊃ φ))) ⊃ (¬¬φ))), from pl1,
+have h6 : prfPA Γ ((¬¬φ) ⊃ ((φ ⊃ (φ ⊃ φ)) ⊃ φ)), from cut h5 h4,
+have h7 : prfPA Γ ((φ ⊃ (φ ⊃ φ)) ⊃ (((φ ⊃ (φ ⊃ φ)) ⊃ φ) ⊃ φ)), from likemp,
+have h8 : prfPA Γ (((φ ⊃ (φ ⊃ φ)) ⊃ φ) ⊃ φ), from mp h7 h1,
+have h9 : prfPA Γ ((¬¬φ) ⊃ φ), from cut h6 h8,
+exact h9
+end
+
+
+lemma dni {Γ : ctxPA agents} {φ : formPA agents} : prfPA Γ (φ ⊃ ¬¬φ) :=
+begin
+have h1 : prfPA Γ ((¬¬(¬φ)) ⊃ (¬φ)), from dne,
+exact mp pl8 h1
+end
+
+
+lemma imp_if_imp_imp {Γ : ctxPA agents} {φ ψ χ : formPA agents} : prfPA Γ (φ ⊃ χ) → prfPA Γ (φ ⊃ (ψ ⊃ χ)) :=
+begin
+intro h1,
+exact mp (mp pl2 (mp pl1 pl1)) h1
+end
+
+
+lemma cut1 {Γ : ctxPA agents} {φ ψ χ θ : formPA agents} :
+  prfPA Γ (θ ⊃ (φ ⊃ ψ)) → prfPA Γ (ψ ⊃ χ) → prfPA Γ (θ ⊃ (φ ⊃ χ)) :=
+begin
+intros h1 h2,
+have h3 : prfPA Γ (φ ⊃ ψ) → prfPA Γ (ψ ⊃ χ) → prfPA Γ (φ ⊃ χ), from cut,
+have h4 : prfPA Γ (θ ⊃ (φ ⊃ ψ)) → prfPA Γ ((φ ⊃ ψ) ⊃ (φ ⊃ χ)) → prfPA Γ (θ ⊃ (φ ⊃ χ)), from cut,
+specialize h4 h1,
+have h5 : prfPA Γ ((φ ⊃ ψ) ⊃ (φ ⊃ χ)), from mp pl2 (mp pl1 h2),
+specialize h4 h5,
+exact h4
+end
+
+
+lemma imp_switch {Γ : ctxPA agents} {φ ψ χ : formPA agents} : prfPA Γ (φ ⊃ (ψ ⊃ χ)) → prfPA Γ (ψ ⊃ (φ ⊃ χ)) :=
+begin
+intro h1,
+have h2 : prfPA Γ (ψ ⊃ ((φ ⊃ ψ) ⊃ (φ ⊃ χ))), from mp pl1 (mp pl2 h1),
+have h3 : prfPA Γ ((ψ ⊃ (φ ⊃ ψ)) ⊃ (ψ ⊃ (φ ⊃ χ))), from mp pl2 h2,
+exact mp h3 pl1
+end
+
+
+lemma l2 {Γ : ctxPA agents} {φ ψ χ : formPA agents} : prfPA Γ ((φ ⊃ (ψ ⊃ χ)) ⊃ (ψ ⊃ (φ ⊃ χ))) :=
+begin
+exact (mp (mp pl2 (cut pl2 hs1)) (mp pl1 pl1))
+end
+
+
+lemma hs2 {Γ : ctxPA agents} {φ ψ χ : formPA agents} :
+  prfPA Γ ((φ ⊃ ψ) ⊃ ((ψ ⊃ χ) ⊃ (φ ⊃ χ))) :=
+begin
+exact (mp l2 hs1)
+end
+
+
+lemma cut2 {Γ : ctxPA agents} {φ ψ χ θ : formPA agents} :
+  prfPA Γ (φ ⊃ ψ) → prfPA Γ (θ ⊃ (ψ ⊃ χ)) → prfPA Γ (θ ⊃ (φ ⊃ χ)) :=
+begin
+intros h1 h2,
+exact imp_switch (cut h1 (imp_switch h2))
+end
+
+
+lemma double_imp {Γ : ctxPA agents} {φ ψ : formPA agents} :
+  prfPA Γ ((φ ⊃ (φ ⊃ ψ)) ⊃ (φ ⊃ ψ)) :=
+begin
+have h1 : prfPA Γ ((φ ⊃ ψ) ⊃ (φ ⊃ ψ)) → prfPA Γ (φ ⊃ ((φ ⊃ ψ) ⊃ ψ)), from imp_switch,
+specialize h1 iden,
+exact mp pl2 h1
+end
+
+
+lemma imp_imp_iff_imp {Γ : ctxPA agents} {θ φ ψ : formPA agents} : 
+  prfPA Γ (θ ⊃ (φ ⊃ (φ ⊃ ψ))) ↔ prfPA Γ (θ ⊃ (φ ⊃ ψ)) :=
+begin
+split,
+{intro h1,
+exact cut h1 double_imp},
+{intro h1,
+exact cut h1 pl1}
+end
+
+
+lemma imp_shift {Γ : ctxPA agents} {θ φ ψ χ : formPA agents} : 
+  prfPA Γ (θ ⊃ (φ ⊃ (ψ ⊃ χ))) ↔ prfPA Γ (θ ⊃ (ψ ⊃ (φ ⊃ χ))) :=
+begin
+split,
+repeat {intro h1, exact cut h1 (cut2 pl1 pl2)}
+end
+
+
+lemma left_and_imp {Γ : ctxPA agents} {φ ψ χ : formPA agents} :
+  prfPA Γ (ψ ⊃ ((φ & ψ) ⊃ χ)) → prfPA Γ ((φ & ψ) ⊃ χ) :=
+begin
+intro h1,
+exact mp double_imp (cut pl6 h1)
+end
+
+
+lemma and_right_imp {Γ : ctxPA agents} {φ ψ χ : formPA agents} : 
+  prfPA Γ ((φ & ψ) ⊃ χ) ↔ prfPA Γ (ψ ⊃ (φ ⊃ χ)) :=
+begin
+split, 
+{intro h1,
+exact mp (cut2 pl1 pl2) (cut1 pl4 h1)},
+intro h1,
+exact left_and_imp (cut2 pl5 h1)
+end
+
+
+lemma not_and_subst {φ ψ χ : formPA agents} {Γ : ctxPA agents} : prfPA Γ (φ ↔ ψ) → (prfPA Γ ¬(χ & φ) ↔ prfPA Γ ¬(χ & ψ)) :=
+begin
+intro h1, split, 
+{intro h2,
+exact mp (mp pl3 (mp pl1 h2)) (cut dne (mp double_imp (cut2 (cut pl6 (mp pl6 h1)) (cut pl5 pl4))))},
+{intro h2,
+exact mp (mp pl3 (mp pl1 h2)) (cut dne (mp double_imp (cut2 (cut pl6 (mp pl5 h1)) (cut pl5 pl4))))},
+end
+
+
+lemma not_contra {Γ : ctxPA agents} {φ : formPA agents} : 
+  prfPA Γ ¬(φ & ¬φ) :=
+begin
+exact mp (mp pl3 (cut dne pl6)) (cut dne pl5)
+end
+
+
+lemma phi_and_true {Γ : ctxPA agents} {φ : formPA agents} : prfPA Γ ((φ&(¬⊥)) ↔ φ) :=
+begin
+exact (mp (mp pl4 pl5) (mp (imp_switch pl4) prtrue))
+end
+
+
+lemma imp_and_and_imp {Γ : ctxPA agents} {φ ψ χ θ : formPA agents} : 
+  prfPA Γ (((φ ⊃ ψ) & (χ ⊃ θ))) → prfPA Γ (((φ & χ) ⊃ (ψ & θ))) :=
+begin
+intro h,
+exact (mp double_imp (cut (cut pl5 (mp pl5 h)) (cut2 (cut pl6 (mp pl6 h)) pl4)))
+end
+
+
+lemma not_contra_equiv_true {Γ : ctxPA agents} {φ : formPA agents} : 
+  prfPA Γ (¬(φ & ¬φ) ↔ ¬⊥) :=
+begin
+exact (mp (mp pl4 (mp pl1 prtrue)) (mp pl1 not_contra))
+end
+
+
+lemma contrapos {Γ : ctxPA agents} {φ ψ : formPA agents} :
+  prfPA Γ ((¬ψ) ⊃ (¬φ)) ↔ prfPA Γ (φ ⊃ ψ) :=
+begin
+split,
+intro h1,
+exact mp pl8 h1,
+intro h1,
+exact mp (cut (cut (mp hs1 dni) (mp hs2 dne)) pl8) h1,
+end
+
+
+lemma iff_not {Γ : ctxPA agents} {φ ψ : formPA agents} :
+  prfPA Γ (φ ↔ ψ) → prfPA Γ (¬ψ ↔ ¬φ) :=
+begin
+intro h1,
+have h2 : prfPA Γ (φ ⊃ ψ), from mp pl5 h1,
+have h3 : prfPA Γ (ψ ⊃ φ), from mp pl6 h1,
+rw ←contrapos at h2,
+rw ←contrapos at h3,
+exact (mp (mp pl4 h2) h3)
+end
+
+
+lemma contra_equiv_false {Γ : ctxPA agents} {φ : formPA agents} : 
+  prfPA Γ ((φ & ¬φ) ↔ ⊥) :=
+begin
+have h1 : prfPA Γ (¬¬⊥ ↔ ¬¬(φ & ¬φ)), from iff_not not_contra_equiv_true,
+exact (mp (mp pl4 (cut dni (cut (mp pl6 h1) dne))) (cut dni (cut (mp pl5 h1) dne)))
+end
+
+
+lemma and_switch {Γ : ctxPA agents} {φ ψ : formPA agents} : prfPA Γ ((φ & ψ) ↔ (ψ & φ)) :=
+begin
+exact (mp (mp pl4 (mp double_imp (cut pl5 (imp_switch (cut pl6 pl4))))) 
+(mp double_imp (cut pl5 (imp_switch (cut pl6 pl4)))))
+end
+
+
+lemma imp_and_imp {Γ : ctxPA agents} {φ ψ χ : formPA agents} : 
+  prfPA Γ (φ ⊃ ψ) → prfPA Γ  ((χ & φ) ⊃ (χ & ψ)) :=
+begin
+intros h1,
+have h2 := imp_and_and_imp,
+specialize h2 (mp (mp pl4 iden) h1), exact h2
+end
+
+
+lemma iff_iff_and_iff {Γ : ctxPA agents} {φ ψ χ θ : formPA agents} : 
+  prfPA Γ (φ ↔ χ) → prfPA Γ (ψ ↔ θ) → prfPA Γ ((φ & ψ) ↔ (χ & θ)) := 
+begin
+intros h1 h2,
+exact mp (mp pl4 (imp_and_and_imp (mp (mp pl4 (mp pl5 h1)) (mp pl5 h2)))) 
+  (imp_and_and_imp (mp (mp pl4 (mp pl6 h1)) (mp pl6 h2)))
+end
+
+lemma and_commute {Γ : ctxPA agents} {φ ψ χ : formPA agents} : prfPA Γ (((φ & ψ) & χ) ↔ (φ & (ψ & χ))) :=
+begin
+exact mp (mp pl4 (mp double_imp (imp_imp_iff_imp.mp 
+  (cut (cut pl5 pl6) (cut2 pl6 (cut1 pl4 (imp_switch (cut (cut pl5 pl5) pl4)))))))) 
+  (mp double_imp (imp_imp_iff_imp.mp (cut (cut pl6 pl5) 
+  (imp_switch (cut pl5 (cut1 pl4 (cut2 (cut pl6 pl6) pl4)))))))
+end
+
+lemma demorgans {Γ : ctxPA agents} {φ ψ : formPA agents} : 
+  prfPA Γ (¬(φ & ψ)) ↔ prfPA Γ (φ ⊃ ¬ψ) :=
+begin
+split,
+intro h1,
+exact (and_right_imp.mp (mp (contrapos.mpr (mp pl5 and_switch)) h1)),
+intro h1,
+exact (mp (contrapos.mpr (mp pl5 and_switch)) (and_right_imp.mpr h1))
+end
+
+lemma explosion {Γ : ctxPA agents} {ψ : formPA agents} : prfPA Γ (⊥ ⊃ ψ) :=
+begin
+apply contrapos.mp, exact (mp pl1 iden)
+end
+
+lemma exfalso {Γ : ctxPA agents} {φ ψ : formPA agents} : prfPA Γ ((φ & ¬φ) ⊃ ψ) :=
+begin
+exact cut not_contra explosion
+end
+
+lemma box_dn {Γ : ctxPA agents} {φ : formPA agents} {a : agents}  : prfPA Γ ((¬K a φ) ↔ ¬(K a (¬¬φ))) :=
+begin
+exact mp (mp pl4 (contrapos.mpr (mp kdist (nec dne)))) (contrapos.mpr (mp kdist (nec dni)))
+end
+
+lemma dual_equiv1 {Γ : ctxPA agents} {φ : formPA agents} {a : agents} : prfPA Γ ((K a φ) ↔ (¬(¬K a ¬(¬φ)))) :=
+begin
+exact mp (mp pl4 (cut (contrapos.mp (mp pl6 box_dn)) dni)) 
+  (cut dne (contrapos.mp (mp pl5 box_dn)))
+end
+
+end PAlemma
